<?xml version="1.0"?>
<!--
#
# Copyright (c) 2008 NEPOMUK Consortium
# Copyright (c) 2012 Sebastian Trueg <trueg@kde.org>
# Copyright (c) 2012 di.me Consortium
#
# All rights reserved, licensed under either CC-BY or BSD.
#
# You are free:
#  * to Share - to copy, distribute and transmit the work
#  * to Remix - to adapt the work
# Under the following conditions:
#  * Attribution - You must attribute the work in the manner specified by the author
#    or licensor (but not in any way that suggests that they endorse you or your use 
#    of the work).
#
# Redistribution and use in source and binary forms, with or without modification, 
# are permitted provided that the following conditions are met:
#  * Redistributions of source code must retain the above copyright notice, this 
#    list of conditions and the following disclaimer.
#  * Redistributions in binary form must reproduce the above copyright notice, this 
#    list of conditions and the following disclaimer in the documentation and/or 
#    other materials provided with the distribution.
#  * Neither the names of the authors nor the names of contributors may
#    be used to endorse or promote products derived from this ontology without 
#    specific prior written permission.
#
# THIS ONTOLOGY IS PROVIDED BY THE AUTHOR ``AS IS'' AND ANY EXPRESS OR
# IMPLIED WARRANTIES, INCLUDING, BUT NOT LIMITED TO, THE IMPLIED WARRANTIES
# OF MERCHANTABILITY AND FITNESS FOR A PARTICULAR PURPOSE ARE DISCLAIMED.
# IN NO EVENT SHALL THE AUTHOR BE LIABLE FOR ANY DIRECT, INDIRECT,
# INCIDENTAL, SPECIAL, EXEMPLARY, OR CONSEQUENTIAL DAMAGES (INCLUDING, BUT
# NOT LIMITED TO, PROCUREMENT OF SUBSTITUTE GOODS OR SERVICES; LOSS OF USE,
# DATA, OR PROFITS; OR BUSINESS INTERRUPTION) HOWEVER CAUSED AND ON ANY
# THEORY OF LIABILITY, WHETHER IN CONTRACT, STRICT LIABILITY, OR TORT
# (INCLUDING NEGLIGENCE OR OTHERWISE) ARISING IN ANY WAY OUT OF THE USE OF
# THIS ONTOLOGY, EVEN IF ADVISED OF THE POSSIBILITY OF SUCH DAMAGE.
#
-->
<rdf:RDF xmlns:nfo="http://www.semanticdesktop.org/ontologies/2007/03/22/nfo#" xmlns:nie="http://www.semanticdesktop.org/ontologies/2007/01/19/nie#" xmlns:xsd="http://www.w3.org/2001/XMLSchema#" xmlns:dc="http://purl.org/dc/elements/1.1/" xmlns:nao="http://www.semanticdesktop.org/ontologies/2007/08/15/nao#" xmlns:nrl="http://www.semanticdesktop.org/ontologies/2007/08/15/nrl#" xmlns:rdf="http://www.w3.org/1999/02/22-rdf-syntax-ns#" xmlns:nco="http://www.semanticdesktop.org/ontologies/2007/03/22/nco#" xmlns:rdfs="http://www.w3.org/2000/01/rdf-schema#" xmlns:owl="http://www.w3.org/2002/07/owl#">
	 <owl:Ontology rdf:about="http://www.w3.org/1999/02/22-rdf-syntax-ns#">
	   <dc:title>NEPOMUK File Ontology (NFO)</dc:title>
	   <dc:description>NEPOMUK File Ontology (NFO) intends to provide vocabulary to express information extracted from various sources. They include files, pieces of sotware and remote hosts. This document gives an overview of NFO and describes its classes and properties. </dc:description>
	 </owl:Ontology>
 
	<rdf:Property rdf:about="http://www.semanticdesktop.org/ontologies/2007/03/22/nfo#horizontalResolution">
		<rdfs:comment>Horizontal resolution of an image (if printed). Expressed in DPI.</rdfs:comment>
		<rdfs:domain>
			<rdfs:Class rdf:about="http://www.semanticdesktop.org/ontologies/2007/03/22/nfo#Image">
				<rdfs:comment>A file containing an image.</rdfs:comment>
				<rdfs:label>Image</rdfs:label>
				<rdfs:subClassOf rdf:resource="http://www.semanticdesktop.org/ontologies/2007/03/22/nfo#Visual" />
			</rdfs:Class>
		</rdfs:domain>
		<rdfs:label>horizontalResolution</rdfs:label>
		<rdfs:range rdf:resource="http://www.w3.org/2001/XMLSchema#integer" />
		<nrl:maxCardinality rdf:datatype="http://www.w3.org/2001/XMLSchema#integer">1</nrl:maxCardinality>
	</rdf:Property>
	<rdf:Property rdf:about="http://www.semanticdesktop.org/ontologies/2007/03/22/nfo#sampleRate">
		<rdfs:comment>The amount of audio samples per second.</rdfs:comment>
		<rdfs:domain>
			<rdfs:Class rdf:about="http://www.semanticdesktop.org/ontologies/2007/03/22/nfo#Audio">
				<rdfs:comment>A file containing audio content</rdfs:comment>
				<rdfs:label>Audio</rdfs:label>
				<rdfs:subClassOf>
					<rdfs:Class rdf:about="http://www.semanticdesktop.org/ontologies/2007/03/22/nfo#Media">
						<rdfs:comment>A piece of media content. This class may be used to express complex media containers with many streams of various media content (both aural and visual).</rdfs:comment>
						<rdfs:label>Media</rdfs:label>
						<rdfs:subClassOf rdf:resource="http://www.semanticdesktop.org/ontologies/2007/01/19/nie#InformationElement" />
					</rdfs:Class>
				</rdfs:subClassOf>
			</rdfs:Class>
		</rdfs:domain>
		<rdfs:label>sampleRate</rdfs:label>
		<rdfs:range rdf:resource="http://www.w3.org/2001/XMLSchema#float" />
		<rdfs:subPropertyOf>
			<rdf:Property rdf:about="http://www.semanticdesktop.org/ontologies/2007/03/22/nfo#rate">
				<rdfs:comment>A common superproperty for all properties specifying the media rate. Examples of subproperties may include frameRate for video and sampleRate for audio. This property is expressed in units per second.</rdfs:comment>
				<rdfs:domain rdf:resource="http://www.semanticdesktop.org/ontologies/2007/03/22/nfo#Media" />
				<rdfs:label>rate</rdfs:label>
				<rdfs:range rdf:resource="http://www.w3.org/2001/XMLSchema#float" />
			</rdf:Property>
		</rdfs:subPropertyOf>
		<nrl:maxCardinality rdf:datatype="http://www.w3.org/2001/XMLSchema#integer">1</nrl:maxCardinality>
	</rdf:Property>
	<rdfs:Class rdf:about="http://www.semanticdesktop.org/ontologies/2007/03/22/nfo#HardDiskPartition">
		<rdfs:comment>A partition on a hard disk</rdfs:comment>
		<rdfs:label>HardDiskPartition</rdfs:label>
		<rdfs:subClassOf rdf:resource="http://www.semanticdesktop.org/ontologies/2007/01/19/nie#DataObject" />
	</rdfs:Class>
	<rdf:Property rdf:about="http://www.semanticdesktop.org/ontologies/2007/03/22/nfo#fileName">
		<rdfs:subPropertyOf rdf:resource="http://www.semanticdesktop.org/ontologies/2007/08/15/nao#prefLabel" />
		<rdfs:comment>Name of the file, together with the extension</rdfs:comment>
		<rdfs:domain>
			<rdfs:Class rdf:about="http://www.semanticdesktop.org/ontologies/2007/03/22/nfo#FileDataObject">
				<rdfs:comment>A resource containing a finite sequence of bytes with arbitrary information, that is available to a computer program and is usually based on some kind of durable storage. A file is durable in the sense that it remains available for programs to use after the current program has finished.</rdfs:comment>
				<rdfs:label>file</rdfs:label>
				<rdfs:subClassOf rdf:resource="http://www.semanticdesktop.org/ontologies/2007/01/19/nie#DataObject" />
			</rdfs:Class>
		</rdfs:domain>
		<rdfs:label>fileName</rdfs:label>
		<nrl:maxCardinality>1</nrl:maxCardinality>
		<rdfs:range rdf:resource="http://www.w3.org/2001/XMLSchema#string" />
	</rdf:Property>
	<rdfs:Class rdf:about="http://www.semanticdesktop.org/ontologies/2007/03/22/nfo#MediaStream">
		<rdfs:comment>A stream of multimedia content, usually contained within a media container such as a movie (containing both audio and video) or a DVD (possibly containing many streams of audio and video). Most common interpretations for such a DataObject include Audio and Video.</rdfs:comment>
		<rdfs:label>MediaStream</rdfs:label>
		<rdfs:subClassOf rdf:resource="http://www.semanticdesktop.org/ontologies/2007/01/19/nie#DataObject" />
	</rdfs:Class>
	<rdfs:Class rdf:about="http://www.semanticdesktop.org/ontologies/2007/03/22/nfo#Presentation">
		<rdfs:comment>A Presentation made by some presentation software (Corel Presentations, OpenOffice Impress, MS Powerpoint etc.)</rdfs:comment>
		<rdfs:label>Presentation</rdfs:label>
		<rdfs:subClassOf>
			<rdfs:Class rdf:about="http://www.semanticdesktop.org/ontologies/2007/03/22/nfo#Document">
				<rdfs:comment>A generic document. A common superclass for all documents on the desktop.</rdfs:comment>
				<rdfs:label>Document</rdfs:label>
				<rdfs:subClassOf rdf:resource="http://www.semanticdesktop.org/ontologies/2007/01/19/nie#InformationElement" />
			</rdfs:Class>
		</rdfs:subClassOf>
	</rdfs:Class>
	<rdf:Property rdf:about="http://www.semanticdesktop.org/ontologies/2007/03/22/nfo#hashAlgorithm">
		<rdfs:comment>Name of the algorithm used to compute the hash value. Examples might include CRC32, MD5, SHA, TTH etc.</rdfs:comment>
		<rdfs:domain>
			<rdfs:Class rdf:about="http://www.semanticdesktop.org/ontologies/2007/03/22/nfo#FileHash">
				<rdfs:comment>A fingerprint of the file, generated by some hashing function.</rdfs:comment>
				<rdfs:label>FileHash</rdfs:label>
				<rdfs:subClassOf rdf:resource="http://www.w3.org/2000/01/rdf-schema#Resource" />
			</rdfs:Class>
		</rdfs:domain>
		<rdfs:label>hashAlgorithm</rdfs:label>
		<rdfs:range rdf:resource="http://www.w3.org/2001/XMLSchema#string" />
		<nrl:maxCardinality rdf:datatype="http://www.w3.org/2001/XMLSchema#integer">1</nrl:maxCardinality>
	</rdf:Property>
	<rdf:Property rdf:about="http://www.semanticdesktop.org/ontologies/2007/03/22/nfo#commentCharacterCount">
		<rdfs:comment>The amount of character in comments i.e. characters ignored by the compiler/interpreter.</rdfs:comment>
		<rdfs:domain>
			<rdfs:Class rdf:about="http://www.semanticdesktop.org/ontologies/2007/03/22/nfo#SourceCode">
				<rdfs:comment>Code in a compilable or interpreted programming language.</rdfs:comment>
				<rdfs:label>SourceCode</rdfs:label>
				<rdfs:subClassOf rdf:resource="http://www.semanticdesktop.org/ontologies/2007/03/22/nfo#PlainTextDocument" />
			</rdfs:Class>
		</rdfs:domain>
		<rdfs:label>commentCharacterCount</rdfs:label>
		<rdfs:range rdf:resource="http://www.w3.org/2001/XMLSchema#integer" />
		<nrl:maxCardinality rdf:datatype="http://www.w3.org/2001/XMLSchema#integer">1</nrl:maxCardinality>
	</rdf:Property>
	<rdfs:Class rdf:about="http://www.semanticdesktop.org/ontologies/2007/03/22/nfo#PlainTextDocument">
		<rdfs:comment>A file containing plain text (ASCII, Unicode or other encodings). Examples may include TXT, HTML, XML, program source code etc.</rdfs:comment>
		<rdfs:label>PlainTextDocument</rdfs:label>
		<rdfs:subClassOf>
			<rdfs:Class rdf:about="http://www.semanticdesktop.org/ontologies/2007/03/22/nfo#TextDocument">
				<rdfs:comment>A text document</rdfs:comment>
				<rdfs:label>TextDocument</rdfs:label>
				<rdfs:subClassOf rdf:resource="http://www.semanticdesktop.org/ontologies/2007/03/22/nfo#Document" />
			</rdfs:Class>
		</rdfs:subClassOf>
	</rdfs:Class>
	<rdf:Property rdf:about="http://www.semanticdesktop.org/ontologies/2007/03/22/nfo#foundry">
		<rdfs:comment>The foundry, the organization that created the font.</rdfs:comment>
		<rdfs:domain>
			<rdfs:Class rdf:about="http://www.semanticdesktop.org/ontologies/2007/03/22/nfo#Font">
				<rdfs:comment>A font.</rdfs:comment>
				<rdfs:label>Font</rdfs:label>
				<rdfs:subClassOf rdf:resource="http://www.semanticdesktop.org/ontologies/2007/01/19/nie#InformationElement" />
			</rdfs:Class>
		</rdfs:domain>
		<rdfs:label>foundry</rdfs:label>
		<rdfs:range rdf:resource="http://www.semanticdesktop.org/ontologies/2007/03/22/nco#Contact" />
		<rdfs:subPropertyOf rdf:resource="http://www.semanticdesktop.org/ontologies/2007/03/22/nco#creator" />
		<nrl:maxCardinality rdf:datatype="http://www.w3.org/2001/XMLSchema#integer">1</nrl:maxCardinality>
	</rdf:Property>
	<nfo:CompressionType rdf:about="http://www.semanticdesktop.org/ontologies/2007/03/22/nfo#losslessCompressionType">
		<rdfs:label>losslessCompressionType</rdfs:label>
	</nfo:CompressionType>
	<rdf:Property rdf:about="http://www.semanticdesktop.org/ontologies/2007/03/22/nfo#sideChannels">
		<rdfs:comment>Number of side channels</rdfs:comment>
		<rdfs:label>sideChannels</rdfs:label>
		<rdfs:range rdf:resource="http://www.w3.org/2001/XMLSchema#integer" />
		<rdfs:subPropertyOf>
			<rdf:Property rdf:about="http://www.semanticdesktop.org/ontologies/2007/03/22/nfo#channels">
				<rdfs:comment>Number of channels. This property is to be used directly if no detailed information is necessary. Otherwise use more detailed subproperties.</rdfs:comment>
				<rdfs:domain rdf:resource="http://www.semanticdesktop.org/ontologies/2007/03/22/nfo#Audio" />
				<rdfs:label>channels</rdfs:label>
				<rdfs:range rdf:resource="http://www.w3.org/2001/XMLSchema#integer" />
				<nrl:maxCardinality rdf:datatype="http://www.w3.org/2001/XMLSchema#integer">1</nrl:maxCardinality>
			</rdf:Property>
		</rdfs:subPropertyOf>
		<nrl:maxCardinality rdf:datatype="http://www.w3.org/2001/XMLSchema#integer">1</nrl:maxCardinality>
	</rdf:Property>
	<rdf:Property rdf:about="http://www.semanticdesktop.org/ontologies/2007/03/22/nfo#interlaceMode">
		<rdfs:comment>True if the image is interlaced, false if not.</rdfs:comment>
		<rdfs:domain>
			<rdfs:Class rdf:about="http://www.semanticdesktop.org/ontologies/2007/03/22/nfo#Visual">
				<rdfs:comment>File containing visual content.</rdfs:comment>
				<rdfs:label>Visual</rdfs:label>
				<rdfs:subClassOf rdf:resource="http://www.semanticdesktop.org/ontologies/2007/03/22/nfo#Media" />
			</rdfs:Class>
		</rdfs:domain>
		<rdfs:label>interlaceMode</rdfs:label>
		<rdfs:range rdf:resource="http://www.w3.org/2001/XMLSchema#boolean" />
		<nrl:maxCardinality rdf:datatype="http://www.w3.org/2001/XMLSchema#integer">1</nrl:maxCardinality>
	</rdf:Property>
	<rdf:Property rdf:about="http://www.semanticdesktop.org/ontologies/2007/03/22/nfo#width">
		<rdfs:comment>Visual content width in pixels.</rdfs:comment>
		<rdfs:domain rdf:resource="http://www.semanticdesktop.org/ontologies/2007/03/22/nfo#Visual" />
		<rdfs:label>width</rdfs:label>
		<rdfs:range rdf:resource="http://www.w3.org/2001/XMLSchema#integer" />
		<nrl:maxCardinality rdf:datatype="http://www.w3.org/2001/XMLSchema#integer">1</nrl:maxCardinality>
	</rdf:Property>
	<rdf:Property rdf:about="http://www.semanticdesktop.org/ontologies/2007/03/22/nfo#frameCount">
		<rdfs:comment>The amount of frames in a video sequence.</rdfs:comment>
		<rdfs:domain>
			<rdfs:Class rdf:about="http://www.semanticdesktop.org/ontologies/2007/03/22/nfo#Video">
				<rdfs:comment>A video file.</rdfs:comment>
				<rdfs:label>Video</rdfs:label>
				<rdfs:subClassOf rdf:resource="http://www.semanticdesktop.org/ontologies/2007/03/22/nfo#Visual" />
			</rdfs:Class>
		</rdfs:domain>
		<rdfs:label>frameCount</rdfs:label>
		<rdfs:range rdf:resource="http://www.w3.org/2001/XMLSchema#integer" />
		<rdfs:subPropertyOf>
			<rdf:Property rdf:about="http://www.semanticdesktop.org/ontologies/2007/03/22/nfo#count">
				<rdfs:comment>A common superproperty for all properties signifying the amount of atomic media data units. Examples of subproperties may include sampleCount and frameCount.</rdfs:comment>
				<rdfs:domain rdf:resource="http://www.semanticdesktop.org/ontologies/2007/03/22/nfo#Media" />
				<rdfs:label>count</rdfs:label>
				<rdfs:range rdf:resource="http://www.w3.org/2001/XMLSchema#integer" />
			</rdf:Property>
		</rdfs:subPropertyOf>
		<nrl:maxCardinality rdf:datatype="http://www.w3.org/2001/XMLSchema#integer">1</nrl:maxCardinality>
	</rdf:Property>
	<rdfs:Class rdf:about="http://www.semanticdesktop.org/ontologies/2007/03/22/nfo#Filesystem">
		<rdfs:comment>A filesystem. Examples of filesystems include hard disk partitions, removable media, but also images thereof stored in files such as ISO.</rdfs:comment>
		<rdfs:label>Filesystem</rdfs:label>
		<rdfs:subClassOf>
			<rdfs:Class rdf:about="http://www.semanticdesktop.org/ontologies/2007/03/22/nfo#DataContainer">
				<rdfs:comment>A superclass for all entities, whose primary purpose is to serve as containers for other data object. They usually don't have any "meaning" by themselves. Examples include folders, archives and optical disc images.</rdfs:comment>
				<rdfs:label>DataContainer</rdfs:label>
				<rdfs:subClassOf rdf:resource="http://www.semanticdesktop.org/ontologies/2007/01/19/nie#InformationElement" />
			</rdfs:Class>
		</rdfs:subClassOf>
	</rdfs:Class>
	<rdf:Property rdf:about="http://www.semanticdesktop.org/ontologies/2007/03/22/nfo#filesystemType">
		<rdfs:comment>Type of filesystem such as ext3 and ntfs.</rdfs:comment>
		<rdfs:domain rdf:resource="http://www.semanticdesktop.org/ontologies/2007/03/22/nfo#Filesystem" />
		<rdfs:range rdf:resource="http://www.w3.org/2001/XMLSchema#string" />
		<rdfs:label>filesystemType</rdfs:label>
		<nrl:maxCardinality rdf:datatype="http://www.w3.org/2001/XMLSchema#integer">1</nrl:maxCardinality>
	</rdf:Property>
	<rdf:Property rdf:about="http://www.semanticdesktop.org/ontologies/2007/03/22/nfo#totalSpace">
		<rdfs:comment>Total storage space of the filesystem, which can be different from nie:contentSize because the latter includes filesystem format overhead.</rdfs:comment>
		<rdfs:domain rdf:resource="http://www.semanticdesktop.org/ontologies/2007/03/22/nfo#Filesystem" />
		<rdfs:range rdf:resource="http://www.w3.org/2001/XMLSchema#integer" />
		<rdfs:label>totalSpace</rdfs:label>
		<nrl:maxCardinality rdf:datatype="http://www.w3.org/2001/XMLSchema#integer">1</nrl:maxCardinality>
	</rdf:Property>
	<rdf:Property rdf:about="http://www.semanticdesktop.org/ontologies/2007/03/22/nfo#freeSpace">
		<rdfs:comment>Unoccupied storage space of the filesystem.</rdfs:comment>
		<rdfs:domain rdf:resource="http://www.semanticdesktop.org/ontologies/2007/03/22/nfo#Filesystem" />
		<rdfs:range rdf:resource="http://www.w3.org/2001/XMLSchema#integer" />
		<rdfs:label>freeSpace</rdfs:label>
		<nrl:maxCardinality rdf:datatype="http://www.w3.org/2001/XMLSchema#integer">1</nrl:maxCardinality>
	</rdf:Property>
	<rdf:Property rdf:about="http://www.semanticdesktop.org/ontologies/2007/03/22/nfo#occupiedSpace">
		<rdfs:comment>Occupied storage space of the filesystem.</rdfs:comment>
		<rdfs:domain rdf:resource="http://www.semanticdesktop.org/ontologies/2007/03/22/nfo#Filesystem" />
		<rdfs:range rdf:resource="http://www.w3.org/2001/XMLSchema#integer" />
		<rdfs:label>occupiedSpace</rdfs:label>
		<nrl:maxCardinality rdf:datatype="http://www.w3.org/2001/XMLSchema#integer">1</nrl:maxCardinality>
	</rdf:Property>
	<rdf:Property rdf:about="http://www.semanticdesktop.org/ontologies/2007/03/22/nfo#uuid">
		<rdfs:subPropertyOf rdf:resource="http://www.semanticdesktop.org/ontologies/2007/01/19/nie#identifier" />
		<rdfs:comment>Universally unique identifier of the filesystem. In the future, this property may have its parent changed to a more generic class.</rdfs:comment>
		<rdfs:domain rdf:resource="http://www.semanticdesktop.org/ontologies/2007/03/22/nfo#Filesystem" />
		<rdfs:range rdf:resource="http://www.w3.org/2001/XMLSchema#string" />
		<rdfs:label>uuid</rdfs:label>
	</rdf:Property>
	<rdf:Property rdf:about="http://www.semanticdesktop.org/ontologies/2007/03/22/nfo#definesFunction">
		<rdfs:comment>A name of a function/method defined in the given source code file.</rdfs:comment>
		<rdfs:domain rdf:resource="http://www.semanticdesktop.org/ontologies/2007/03/22/nfo#SourceCode" />
		<rdfs:label>definesFunction</rdfs:label>
		<rdfs:range rdf:resource="http://www.w3.org/2001/XMLSchema#string" />
	</rdf:Property>
	<rdf:Property rdf:about="http://www.semanticdesktop.org/ontologies/2007/03/22/nfo#permissions">
		<rdfs:comment>A string containing the permissions of a file. A feature common in many UNIX-like operating systems.</rdfs:comment>
		<rdfs:domain rdf:resource="http://www.semanticdesktop.org/ontologies/2007/03/22/nfo#FileDataObject" />
		<rdfs:label>permissions</rdfs:label>
		<rdfs:range rdf:resource="http://www.w3.org/2001/XMLSchema#string" />
		<nrl:maxCardinality rdf:datatype="http://www.w3.org/2001/XMLSchema#integer">1</nrl:maxCardinality>
	</rdf:Property>
	<rdf:Property rdf:about="http://www.semanticdesktop.org/ontologies/2007/03/22/nfo#lineCount">
		<rdfs:comment>The amount of lines in a text document</rdfs:comment>
		<rdfs:domain rdf:resource="http://www.semanticdesktop.org/ontologies/2007/03/22/nfo#TextDocument" />
		<rdfs:label>lineCount</rdfs:label>
		<rdfs:range rdf:resource="http://www.w3.org/2001/XMLSchema#integer" />
		<nrl:maxCardinality rdf:datatype="http://www.w3.org/2001/XMLSchema#integer">1</nrl:maxCardinality>
	</rdf:Property>
	<rdfs:Class rdf:about="http://www.semanticdesktop.org/ontologies/2007/03/22/nfo#SoftwareItem">
		<rdfs:comment>A DataObject representing a piece of software. Examples of interpretations of a SoftwareItem include an Application and an OperatingSystem.</rdfs:comment>
		<rdfs:label>SoftwareItem</rdfs:label>
		<rdfs:subClassOf rdf:resource="http://www.semanticdesktop.org/ontologies/2007/01/19/nie#DataObject" />
	</rdfs:Class>
	<rdf:Property rdf:about="http://www.semanticdesktop.org/ontologies/2007/03/22/nfo#wordCount">
		<rdfs:comment>The amount of words in a text document.</rdfs:comment>
		<rdfs:domain rdf:resource="http://www.semanticdesktop.org/ontologies/2007/03/22/nfo#TextDocument" />
		<rdfs:label>wordCount</rdfs:label>
		<rdfs:range rdf:resource="http://www.w3.org/2001/XMLSchema#integer" />
		<nrl:maxCardinality rdf:datatype="http://www.w3.org/2001/XMLSchema#integer">1</nrl:maxCardinality>
	</rdf:Property>
	<rdf:Property rdf:about="http://www.semanticdesktop.org/ontologies/2007/03/22/nfo#bookmarks">
		<rdfs:comment>The address of the linked object. Usually a web URI.</rdfs:comment>
		<rdfs:domain>
			<rdfs:Class rdf:about="http://www.semanticdesktop.org/ontologies/2007/03/22/nfo#Bookmark">
				<rdfs:comment>A bookmark of a webbrowser. Use nie:title for the name/label, nie:contentCreated to represent the date when the user added the bookmark, and nie:contentLastModified for modifications. nfo:bookmarks to store the link.</rdfs:comment>
				<rdfs:label>Bookmark</rdfs:label>
				<rdfs:subClassOf rdf:resource="http://www.semanticdesktop.org/ontologies/2007/01/19/nie#InformationElement" />
			</rdfs:Class>
		</rdfs:domain>
		<rdfs:label>link</rdfs:label>
		<rdfs:range rdf:resource="http://www.semanticdesktop.org/ontologies/2007/01/19/nie#DataObject" />
		<rdfs:subPropertyOf rdf:resource="http://www.semanticdesktop.org/ontologies/2007/01/19/nie#links" />
		<nrl:cardinality rdf:datatype="http://www.w3.org/2001/XMLSchema#integer">1</nrl:cardinality>
	</rdf:Property>
	<rdf:Property rdf:about="http://www.semanticdesktop.org/ontologies/2007/03/22/nfo#characterPosition">
		<rdfs:comment>Character position of the bookmark.</rdfs:comment>
		<rdfs:domain rdf:resource="http://www.semanticdesktop.org/ontologies/2007/03/22/nfo#Bookmark" />
		<rdfs:label>characterPosition</rdfs:label>
		<rdfs:range rdf:resource="http://www.w3.org/2001/XMLSchema#integer" />
		<nrl:maxCardinality rdf:datatype="http://www.w3.org/2001/XMLSchema#integer">1</nrl:maxCardinality>
	</rdf:Property>
	<rdf:Property rdf:about="http://www.semanticdesktop.org/ontologies/2007/03/22/nfo#pageNumber">
		<rdfs:comment>Page linked by the bookmark.</rdfs:comment>
		<rdfs:domain rdf:resource="http://www.semanticdesktop.org/ontologies/2007/03/22/nfo#Bookmark" />
		<rdfs:label>pageNumber</rdfs:label>
		<rdfs:range rdf:resource="http://www.w3.org/2001/XMLSchema#integer" />
		<nrl:maxCardinality rdf:datatype="http://www.w3.org/2001/XMLSchema#integer">1</nrl:maxCardinality>
	</rdf:Property>
	<rdf:Property rdf:about="http://www.semanticdesktop.org/ontologies/2007/03/22/nfo#streamPosition">
		<rdfs:comment>Stream position of the bookmark, suitable for e.g. audio books. Expressed in milliseconds</rdfs:comment>
		<rdfs:domain rdf:resource="http://www.semanticdesktop.org/ontologies/2007/03/22/nfo#Bookmark" />
		<rdfs:label>streamPosition</rdfs:label>
		<rdfs:range rdf:resource="http://www.w3.org/2001/XMLSchema#integer" />
		<nrl:maxCardinality rdf:datatype="http://www.w3.org/2001/XMLSchema#integer">1</nrl:maxCardinality>
	</rdf:Property>
	<rdfs:Class rdf:about="http://www.semanticdesktop.org/ontologies/2007/03/22/nfo#RemotePortAddress">
		<rdfs:comment>An address specifying a remote host and port. Such an address can be interpreted in many ways (examples of such interpretations include mailboxes, websites, remote calendars or filesystems), depending on an interpretation, various kinds of data may be extracted from such an address.</rdfs:comment>
		<rdfs:label>RemotePortAddress</rdfs:label>
		<rdfs:subClassOf rdf:resource="http://www.semanticdesktop.org/ontologies/2007/01/19/nie#DataObject" />
	</rdfs:Class>
	<rdfs:Class rdf:about="http://www.semanticdesktop.org/ontologies/2007/03/22/nfo#Attachment">
		<rdfs:comment>A file attached to another data object. Many data formats allow for attachments: emails, vcards, ical events, id3 and exif...</rdfs:comment>
		<rdfs:label>Attachment</rdfs:label>
		<rdfs:subClassOf>
			<rdfs:Class rdf:about="http://www.semanticdesktop.org/ontologies/2007/03/22/nfo#EmbeddedFileDataObject">
				<rdfs:comment>A file embedded in another data object. There are many ways in which a file may be embedded in another one. Use this class directly only in cases if none of the subclasses gives a better description of your case.</rdfs:comment>
				<rdfs:label>EmbeddedFileDataObject</rdfs:label>
				<rdfs:subClassOf rdf:resource="http://www.semanticdesktop.org/ontologies/2007/03/22/nfo#FileDataObject" />
			</rdfs:Class>
		</rdfs:subClassOf>
	</rdfs:Class>
	<rdf:Property rdf:about="http://www.semanticdesktop.org/ontologies/2007/03/22/nfo#characterCount">
		<rdfs:comment>The amount of characters in the document.</rdfs:comment>
		<rdfs:domain rdf:resource="http://www.semanticdesktop.org/ontologies/2007/03/22/nfo#TextDocument" />
		<rdfs:label>characterCount</rdfs:label>
		<rdfs:range rdf:resource="http://www.w3.org/2001/XMLSchema#integer" />
		<nrl:maxCardinality rdf:datatype="http://www.w3.org/2001/XMLSchema#integer">1</nrl:maxCardinality>
	</rdf:Property>
	<rdf:Property rdf:about="http://www.semanticdesktop.org/ontologies/2007/03/22/nfo#fileLastAccessed">
		<rdfs:comment>Time when the file was last accessed.</rdfs:comment>
		<rdfs:domain rdf:resource="http://www.semanticdesktop.org/ontologies/2007/03/22/nfo#FileDataObject" />
		<rdfs:label>fileLastAccessed</rdfs:label>
		<rdfs:range rdf:resource="http://www.w3.org/2001/XMLSchema#dateTime" />
		<rdfs:subPropertyOf rdf:resource="http://purl.org/dc/elements/1.1/date" />
		<nrl:maxCardinality rdf:datatype="http://www.w3.org/2001/XMLSchema#integer">1</nrl:maxCardinality>
	</rdf:Property>
	<rdf:Property rdf:about="http://www.semanticdesktop.org/ontologies/2007/03/22/nfo#supercedes">
		<rdfs:comment>States that a piece of software supercedes another piece of software.</rdfs:comment>
		<rdfs:domain>
			<rdfs:Class rdf:about="http://www.semanticdesktop.org/ontologies/2007/03/22/nfo#Software">
				<rdfs:comment>A piece of software. Examples may include applications and the operating system. This interpretation most commonly applies to SoftwareItems.</rdfs:comment>
				<rdfs:label>Software</rdfs:label>
				<rdfs:subClassOf rdf:resource="http://www.semanticdesktop.org/ontologies/2007/01/19/nie#InformationElement" />
				<rdfs:subClassOf rdf:resource="http://www.semanticdesktop.org/ontologies/2007/08/15/nao#Agent" />
			</rdfs:Class>
		</rdfs:domain>
		<rdfs:label>supercedes</rdfs:label>
		<rdfs:range rdf:resource="http://www.semanticdesktop.org/ontologies/2007/03/22/nfo#Software" />
	</rdf:Property>
	<rdf:Property rdf:about="http://www.semanticdesktop.org/ontologies/2007/03/22/nfo#programmingLanguage">
		<rdfs:comment>Indicates the name of the programming language this source code file is written in. Examples might include 'C', 'C++', 'Java' etc.</rdfs:comment>
		<rdfs:domain rdf:resource="http://www.semanticdesktop.org/ontologies/2007/03/22/nfo#SourceCode" />
		<rdfs:label>programmingLanguage</rdfs:label>
		<rdfs:range rdf:resource="http://www.w3.org/2001/XMLSchema#string" />
	</rdf:Property>
	<rdfs:Class rdf:about="http://www.semanticdesktop.org/ontologies/2007/03/22/nfo#Application">
		<rdfs:comment>An application</rdfs:comment>
		<rdfs:label>Application</rdfs:label>
		<rdfs:subClassOf rdf:resource="http://www.semanticdesktop.org/ontologies/2007/03/22/nfo#Software" />
	</rdfs:Class>
	<rdf:Property rdf:about="http://www.semanticdesktop.org/ontologies/2007/03/22/nfo#sampleCount">
		<rdfs:comment>The amount of samples in an audio clip.</rdfs:comment>
		<rdfs:domain rdf:resource="http://www.semanticdesktop.org/ontologies/2007/03/22/nfo#Audio" />
		<rdfs:label>sampleCount</rdfs:label>
		<rdfs:range rdf:resource="http://www.w3.org/2001/XMLSchema#integer" />
		<rdfs:subPropertyOf rdf:resource="http://www.semanticdesktop.org/ontologies/2007/03/22/nfo#count" />
		<nrl:maxCardinality rdf:datatype="http://www.w3.org/2001/XMLSchema#integer">1</nrl:maxCardinality>
	</rdf:Property>
	<rdf:Property rdf:about="http://www.semanticdesktop.org/ontologies/2007/03/22/nfo#height">
		<rdfs:comment>Visual content height in pixels.</rdfs:comment>
		<rdfs:domain rdf:resource="http://www.semanticdesktop.org/ontologies/2007/03/22/nfo#Visual" />
		<rdfs:label>height</rdfs:label>
		<rdfs:range rdf:resource="http://www.w3.org/2001/XMLSchema#integer" />
		<nrl:maxCardinality rdf:datatype="http://www.w3.org/2001/XMLSchema#integer">1</nrl:maxCardinality>
	</rdf:Property>
	<rdf:Property rdf:about="http://www.semanticdesktop.org/ontologies/2007/03/22/nfo#frontChannels">
		<rdfs:comment>Number of front channels.</rdfs:comment>
		<rdfs:label>frontChannels</rdfs:label>
		<rdfs:range rdf:resource="http://www.w3.org/2001/XMLSchema#integer" />
		<rdfs:subPropertyOf rdf:resource="http://www.semanticdesktop.org/ontologies/2007/03/22/nfo#channels" />
		<nrl:maxCardinality rdf:datatype="http://www.w3.org/2001/XMLSchema#integer">1</nrl:maxCardinality>
	</rdf:Property>
	<rdfs:Class rdf:about="http://www.semanticdesktop.org/ontologies/2007/03/22/nfo#FilesystemImage">
		<nao:deprecated rdf:datatype="http://www.w3.org/2001/XMLSchema#boolean">true</nao:deprecated>
		<rdfs:comment>An image of a filesystem. Instances of this class may include CD images, DVD images or hard disk partition images created by various pieces of software (e.g. Norton Ghost). Deprecated in favor of nfo:Filesystem.</rdfs:comment>
		<rdfs:label>FilesystemImage</rdfs:label>
		<rdfs:subClassOf rdf:resource="http://www.semanticdesktop.org/ontologies/2007/03/22/nfo#Filesystem" />
	</rdfs:Class>
	<rdf:Property rdf:about="http://www.semanticdesktop.org/ontologies/2007/03/22/nfo#rearChannels">
		<rdfs:comment>Number of rear channels.</rdfs:comment>
		<rdfs:label>rearChannels</rdfs:label>
		<rdfs:range rdf:resource="http://www.w3.org/2001/XMLSchema#integer" />
		<rdfs:subPropertyOf rdf:resource="http://www.semanticdesktop.org/ontologies/2007/03/22/nfo#channels" />
		<nrl:maxCardinality rdf:datatype="http://www.w3.org/2001/XMLSchema#integer">1</nrl:maxCardinality>
	</rdf:Property>
	<rdf:Property rdf:about="http://www.semanticdesktop.org/ontologies/2007/03/22/nfo#bitsPerSample">
		<rdfs:comment>Amount of bits in each audio sample.</rdfs:comment>
		<rdfs:domain rdf:resource="http://www.semanticdesktop.org/ontologies/2007/03/22/nfo#Audio" />
		<rdfs:label>bitsPerSample</rdfs:label>
		<rdfs:range rdf:resource="http://www.w3.org/2001/XMLSchema#integer" />
		<rdfs:subPropertyOf>
			<rdf:Property rdf:about="http://www.semanticdesktop.org/ontologies/2007/03/22/nfo#bitDepth">
				<rdfs:comment>A common superproperty for all properties signifying the amount of bits for an atomic unit of data. Examples of subproperties may include bitsPerSample and bitsPerPixel</rdfs:comment>
				<rdfs:domain rdf:resource="http://www.semanticdesktop.org/ontologies/2007/03/22/nfo#Media" />
				<rdfs:label>bitDepth</rdfs:label>
				<rdfs:range rdf:resource="http://www.w3.org/2000/01/rdf-schema#Literal" />
				<nrl:maxCardinality rdf:datatype="http://www.w3.org/2001/XMLSchema#integer">1</nrl:maxCardinality>
			</rdf:Property>
		</rdfs:subPropertyOf>
		<nrl:maxCardinality rdf:datatype="http://www.w3.org/2001/XMLSchema#integer">1</nrl:maxCardinality>
	</rdf:Property>
	<rdfs:Class rdf:about="http://www.semanticdesktop.org/ontologies/2007/03/22/nfo#HtmlDocument">
		<rdfs:comment>A HTML document, may contain links to other files.</rdfs:comment>
		<rdfs:label>HtmlDocument</rdfs:label>
		<rdfs:subClassOf rdf:resource="http://www.semanticdesktop.org/ontologies/2007/03/22/nfo#PlainTextDocument" />
	</rdfs:Class>
	<rdf:Property rdf:about="http://www.semanticdesktop.org/ontologies/2007/03/22/nfo#duration">
		<rdfs:comment>Duration of a media piece.</rdfs:comment>
		<rdfs:domain rdf:resource="http://www.semanticdesktop.org/ontologies/2007/03/22/nfo#Media" />
		<rdfs:label>duration</rdfs:label>
		<rdfs:range rdf:resource="http://www.w3.org/2001/XMLSchema#duration" />
		<nrl:maxCardinality rdf:datatype="http://www.w3.org/2001/XMLSchema#integer">1</nrl:maxCardinality>
	</rdf:Property>
	<rdf:Property rdf:about="http://www.semanticdesktop.org/ontologies/2007/03/22/nfo#lfeChannels">
		<rdfs:comment>Number of Low Frequency Expansion (subwoofer) channels.</rdfs:comment>
		<rdfs:label>lfeChannels</rdfs:label>
		<rdfs:range rdf:resource="http://www.w3.org/2001/XMLSchema#integer" />
		<rdfs:subPropertyOf rdf:resource="http://www.semanticdesktop.org/ontologies/2007/03/22/nfo#channels" />
		<nrl:maxCardinality rdf:datatype="http://www.w3.org/2001/XMLSchema#integer">1</nrl:maxCardinality>
	</rdf:Property>
	<rdf:Property rdf:about="http://www.semanticdesktop.org/ontologies/2007/03/22/nfo#hasMediaStream">
		<rdfs:comment>Connects a media container with a single media stream contained within.</rdfs:comment>
		<rdfs:domain rdf:resource="http://www.semanticdesktop.org/ontologies/2007/03/22/nfo#Media" />
		<rdfs:label>hasMediaStream</rdfs:label>
		<rdfs:range rdf:resource="http://www.semanticdesktop.org/ontologies/2007/01/19/nie#DataObject" />
		<rdfs:subPropertyOf rdf:resource="http://www.semanticdesktop.org/ontologies/2007/01/19/nie#hasPart" />
	</rdf:Property>
	<rdfs:Class rdf:about="http://www.semanticdesktop.org/ontologies/2007/03/22/nfo#Spreadsheet">
		<rdfs:comment>A spreadsheet, created by a spreadsheet application. Examples might include Gnumeric, OpenOffice Calc or MS Excel.</rdfs:comment>
		<rdfs:label>Spreadsheet</rdfs:label>
		<rdfs:subClassOf rdf:resource="http://www.semanticdesktop.org/ontologies/2007/03/22/nfo#Document" />
	</rdfs:Class>
	<rdf:Property rdf:about="http://www.semanticdesktop.org/ontologies/2007/03/22/nfo#isPasswordProtected">
		<rdfs:comment>States if a given resource is password-protected.</rdfs:comment>
		<rdfs:domain>
			<rdfs:Class rdf:about="http://www.semanticdesktop.org/ontologies/2007/03/22/nfo#ArchiveItem">
				<rdfs:comment>A file entity inside an archive.</rdfs:comment>
				<rdfs:label>ArchiveItem</rdfs:label>
				<rdfs:subClassOf rdf:resource="http://www.semanticdesktop.org/ontologies/2007/03/22/nfo#EmbeddedFileDataObject" />
			</rdfs:Class>
		</rdfs:domain>
		<rdfs:label>isPasswordProtected</rdfs:label>
		<rdfs:range rdf:resource="http://www.w3.org/2001/XMLSchema#boolean" />
		<nrl:maxCardinality rdf:datatype="http://www.w3.org/2001/XMLSchema#integer">1</nrl:maxCardinality>
	</rdf:Property>
	<rdf:Property rdf:about="http://www.semanticdesktop.org/ontologies/2007/03/22/nfo#hashValue">
		<rdfs:comment>The actual value of the hash.</rdfs:comment>
		<rdfs:domain rdf:resource="http://www.semanticdesktop.org/ontologies/2007/03/22/nfo#FileHash" />
		<rdfs:label>hashValue</rdfs:label>
		<rdfs:range rdf:resource="http://www.w3.org/2001/XMLSchema#string" />
		<nrl:cardinality rdf:datatype="http://www.w3.org/2001/XMLSchema#integer">1</nrl:cardinality>
	</rdf:Property>
	<nfo:EncryptionStatus rdf:about="http://www.semanticdesktop.org/ontologies/2007/03/22/nfo#encryptedStatus">
		<rdfs:label>EncryptedStatus</rdfs:label>
	</nfo:EncryptionStatus>
	<rdf:Property rdf:about="http://www.semanticdesktop.org/ontologies/2007/03/22/nfo#uncompressedSize">
		<rdfs:comment>Uncompressed size of the content of a compressed file.</rdfs:comment>
		<rdfs:domain>
			<rdfs:Class rdf:about="http://www.semanticdesktop.org/ontologies/2007/03/22/nfo#Archive">
				<rdfs:comment>A compressed file. May contain other files or folder inside. </rdfs:comment>
				<rdfs:label>Archive</rdfs:label>
				<rdfs:subClassOf rdf:resource="http://www.semanticdesktop.org/ontologies/2007/03/22/nfo#DataContainer" />
			</rdfs:Class>
		</rdfs:domain>
		<rdfs:label>uncompressedSize</rdfs:label>
		<rdfs:range rdf:resource="http://www.w3.org/2001/XMLSchema#integer" />
		<nrl:maxCardinality rdf:datatype="http://www.w3.org/2001/XMLSchema#integer">1</nrl:maxCardinality>
	</rdf:Property>
	<rdf:Property rdf:about="http://www.semanticdesktop.org/ontologies/2007/03/22/nfo#deletionDate">
		<rdfs:comment>The date and time of the deletion.</rdfs:comment>
		<rdfs:domain>
			<rdfs:Class rdf:about="http://www.semanticdesktop.org/ontologies/2007/03/22/nfo#DeletedResource">
				<rdfs:comment>A file entity that has been deleted from the original source. Usually such entities are stored within various kinds of 'Trash' or 'Recycle Bin' folders.</rdfs:comment>
				<rdfs:label>DeletedResource</rdfs:label>
				<rdfs:subClassOf rdf:resource="http://www.semanticdesktop.org/ontologies/2007/03/22/nfo#FileDataObject" />
			</rdfs:Class>
		</rdfs:domain>
		<rdfs:label>deletionDate</rdfs:label>
		<rdfs:range rdf:resource="http://www.w3.org/2001/XMLSchema#dateTime" />
		<nrl:maxCardinality rdf:datatype="http://www.w3.org/2001/XMLSchema#integer">1</nrl:maxCardinality>
	</rdf:Property>
	<rdfs:Class rdf:about="http://www.semanticdesktop.org/ontologies/2007/03/22/nfo#MindMap">
		<rdfs:comment>A MindMap, created by a mind-mapping utility. Examples might include FreeMind or mind mapper.</rdfs:comment>
		<rdfs:label>MindMap</rdfs:label>
		<rdfs:subClassOf rdf:resource="http://www.semanticdesktop.org/ontologies/2007/03/22/nfo#Document" />
	</rdfs:Class>
	<rdfs:Class rdf:about="http://www.semanticdesktop.org/ontologies/2007/03/22/nfo#SoftwareService">
		<rdfs:comment>A service published by a piece of software, either by an operating system or an application. Examples of such services may include calendar, addressbook and mailbox managed by a PIM application. This category is introduced to distinguish between data available directly from the applications (Via some Interprocess Communication Mechanisms) and data available from files on a disk. In either case both DataObjects would receive a similar interpretation (e.g. a Mailbox) and wouldn't differ on the content level.</rdfs:comment>
		<rdfs:label>SoftwareService</rdfs:label>
		<rdfs:subClassOf rdf:resource="http://www.semanticdesktop.org/ontologies/2007/01/19/nie#DataObject" />
	</rdfs:Class>
	<nfo:EncryptionStatus rdf:about="http://www.semanticdesktop.org/ontologies/2007/03/22/nfo#decryptedStatus">
		<rdfs:label>DecryptedStatus</rdfs:label>
	</nfo:EncryptionStatus>
	<rdf:Property rdf:about="http://www.semanticdesktop.org/ontologies/2007/03/22/nfo#originalLocation">
		<rdfs:comment>The original location of the deleted resource.</rdfs:comment>
		<rdfs:domain rdf:resource="http://www.semanticdesktop.org/ontologies/2007/03/22/nfo#DeletedResource" />
		<rdfs:label>originalLocation</rdfs:label>
		<rdfs:range rdf:resource="http://www.w3.org/2001/XMLSchema#string" />
		<nrl:maxCardinality rdf:datatype="http://www.w3.org/2001/XMLSchema#integer">1</nrl:maxCardinality>
	</rdf:Property>
	<rdfs:Class rdf:about="http://www.semanticdesktop.org/ontologies/2007/03/22/nfo#Website">
		<rdfs:comment>A website, usually a container for remote resources, that may be interpreted as HTMLDocuments, images or other types of content.</rdfs:comment>
		<rdfs:label>Website</rdfs:label>
		<rdfs:subClassOf rdf:resource="http://www.semanticdesktop.org/ontologies/2007/01/19/nie#InformationElement" />
	</rdfs:Class>
	<rdfs:Class rdf:about="http://www.semanticdesktop.org/ontologies/2007/03/22/nfo#VectorImage">
		<rdfs:label>VectorImage</rdfs:label>
		<rdfs:subClassOf rdf:resource="http://www.semanticdesktop.org/ontologies/2007/03/22/nfo#Image" />
	</rdfs:Class>
	<rdfs:Class rdf:about="http://www.semanticdesktop.org/ontologies/2007/03/22/nfo#Cursor">
		<rdfs:comment>A Cursor.</rdfs:comment>
		<rdfs:label>Cursor</rdfs:label>
		<rdfs:subClassOf>
			<rdfs:Class rdf:about="http://www.semanticdesktop.org/ontologies/2007/03/22/nfo#RasterImage">
				<rdfs:comment>A raster image.</rdfs:comment>
				<rdfs:label>RasterImage</rdfs:label>
				<rdfs:subClassOf rdf:resource="http://www.semanticdesktop.org/ontologies/2007/03/22/nfo#Image" />
			</rdfs:Class>
		</rdfs:subClassOf>
	</rdfs:Class>
	<rdf:Property rdf:about="http://www.semanticdesktop.org/ontologies/2007/03/22/nfo#hasMediaFileListEntry">
		<rdfs:comment>This property is intended to point to an RDF list of MediaFiles.</rdfs:comment>
		<rdfs:domain>
			<rdfs:Class rdf:about="http://www.semanticdesktop.org/ontologies/2007/03/22/nfo#MediaList">
				<rdfs:comment>A file containing a list of media files.e.g. a playlist</rdfs:comment>
				<rdfs:label>MediaList</rdfs:label>
				<rdfs:subClassOf rdf:resource="http://www.semanticdesktop.org/ontologies/2007/01/19/nie#InformationElement" />
			</rdfs:Class>
		</rdfs:domain>
		<rdfs:label>hasMediaFileListEntry</rdfs:label>
		<rdfs:range>
			<rdfs:Class rdf:about="http://www.semanticdesktop.org/ontologies/2007/03/22/nfo#MediaFileListEntry">
				<rdfs:comment>A single node in the list of media files contained within an MediaList instance. This class is intended to provide a type all those links have. In valid NRL untyped resources cannot be linked. There are no properties defined for this class but the application may expect rdf:first and rdf:last links. The former points to the DataObject instance, interpreted as Media the latter points at another MediaFileListEntr. At the end of the list there is a link to rdf:nil.</rdfs:comment>
				<rdfs:label>MediaFileListEntry</rdfs:label>
				<rdfs:subClassOf rdf:resource="http://www.w3.org/2000/01/rdf-schema#Resource" />
			</rdfs:Class>
		</rdfs:range>
	</rdf:Property>
	<rdfs:Class rdf:about="http://www.semanticdesktop.org/ontologies/2007/03/22/nfo#BookmarkFolder">
		<rdfs:comment>A folder with bookmarks of a webbrowser. Use nfo:containsBookmark to relate Bookmarks. Folders can contain subfolders, use containsBookmarkFolder to relate them.</rdfs:comment>
		<rdfs:label>Bookmark Folder</rdfs:label>
		<rdfs:subClassOf rdf:resource="http://www.semanticdesktop.org/ontologies/2007/01/19/nie#InformationElement" />
	</rdfs:Class>
	<rdf:Property rdf:about="http://www.semanticdesktop.org/ontologies/2007/03/22/nfo#colorDepth">
		<rdfs:comment>Amount of bits used to express the color of each pixel.</rdfs:comment>
		<rdfs:domain rdf:resource="http://www.semanticdesktop.org/ontologies/2007/03/22/nfo#Visual" />
		<rdfs:label>colorDepth</rdfs:label>
		<rdfs:range rdf:resource="http://www.w3.org/2001/XMLSchema#integer" />
		<rdfs:subPropertyOf rdf:resource="http://www.semanticdesktop.org/ontologies/2007/03/22/nfo#bitDepth" />
		<nrl:maxCardinality rdf:datatype="http://www.w3.org/2001/XMLSchema#integer">1</nrl:maxCardinality>
	</rdf:Property>
	<rdf:Property rdf:about="http://www.semanticdesktop.org/ontologies/2007/03/22/nfo#averageBitrate">
		<rdfs:comment>The average overall bitrate of a media container. (i.e. the size of the piece of media in bits, divided by it's duration expressed in seconds).</rdfs:comment>
		<rdfs:domain rdf:resource="http://www.semanticdesktop.org/ontologies/2007/03/22/nfo#Media" />
		<rdfs:label>averageBitrate</rdfs:label>
		<rdfs:range rdf:resource="http://www.w3.org/2001/XMLSchema#float" />
		<rdfs:subPropertyOf rdf:resource="http://www.semanticdesktop.org/ontologies/2007/03/22/nfo#rate" />
		<nrl:maxCardinality rdf:datatype="http://www.w3.org/2001/XMLSchema#integer">1</nrl:maxCardinality>
	</rdf:Property>
	<rdfs:Class rdf:about="http://www.semanticdesktop.org/ontologies/2007/03/22/nfo#Icon">
		<rdfs:comment>An Icon (regardless of whether it's a raster or a vector icon. A resource representing an icon could have two types (Icon and Raster, or Icon and Vector) if required.</rdfs:comment>
		<rdfs:label>Icon</rdfs:label>
		<rdfs:subClassOf rdf:resource="http://www.semanticdesktop.org/ontologies/2007/03/22/nfo#Image" />
	</rdfs:Class>
	<rdf:Property rdf:about="http://www.semanticdesktop.org/ontologies/2007/03/22/nfo#fileOwner">
		<rdfs:comment>The owner of the file as defined by the file system access rights feature.</rdfs:comment>
		<rdfs:domain rdf:resource="http://www.semanticdesktop.org/ontologies/2007/03/22/nfo#FileDataObject" />
		<rdfs:label>fileOwner</rdfs:label>
		<rdfs:range rdf:resource="http://www.semanticdesktop.org/ontologies/2007/03/22/nco#Contact" />
		<nrl:maxCardinality rdf:datatype="http://www.w3.org/2001/XMLSchema#integer">1</nrl:maxCardinality>
	</rdf:Property>
	<rdf:Property rdf:about="http://www.semanticdesktop.org/ontologies/2007/03/22/nfo#aspectRatio">
		<rdfs:comment>Visual content aspect ratio. (Width divided by Height)</rdfs:comment>
		<rdfs:domain rdf:resource="http://www.semanticdesktop.org/ontologies/2007/03/22/nfo#Visual" />
		<rdfs:label>aspectRatio</rdfs:label>
		<rdfs:range rdf:resource="http://www.w3.org/2001/XMLSchema#float" />
		<nrl:maxCardinality rdf:datatype="http://www.w3.org/2001/XMLSchema#integer">1</nrl:maxCardinality>
	</rdf:Property>
	<rdf:Property rdf:about="http://www.semanticdesktop.org/ontologies/2007/03/22/nfo#containsBookmarkFolder">
		<rdfs:comment>The folder contains a bookmark folder.</rdfs:comment>
		<rdfs:domain rdf:resource="http://www.semanticdesktop.org/ontologies/2007/03/22/nfo#BookmarkFolder" />
		<rdfs:label>contains folder</rdfs:label>
		<rdfs:range rdf:resource="http://www.semanticdesktop.org/ontologies/2007/03/22/nfo#BookmarkFolder" />
		<rdfs:subPropertyOf rdf:resource="http://www.semanticdesktop.org/ontologies/2007/01/19/nie#hasLogicalPart" />
	</rdf:Property>
	<rdf:Property rdf:about="http://www.semanticdesktop.org/ontologies/2007/03/22/nfo#belongsToContainer">
		<rdfs:comment>Models the containment relations between Files and Folders (or CompressedFiles).</rdfs:comment>
		<rdfs:domain rdf:resource="http://www.semanticdesktop.org/ontologies/2007/01/19/nie#DataObject" />
		<rdfs:label>belongsToContainer</rdfs:label>
		<rdfs:range rdf:resource="http://www.semanticdesktop.org/ontologies/2007/03/22/nfo#DataContainer" />
		<rdfs:subPropertyOf rdf:resource="http://www.semanticdesktop.org/ontologies/2007/01/19/nie#isPartOf" />
	</rdf:Property>
	<rdf:Property rdf:about="http://www.semanticdesktop.org/ontologies/2007/03/22/nfo#verticalResolution">
		<rdfs:comment>Vertical resolution of an Image (if printed). Expressed in DPI</rdfs:comment>
		<rdfs:domain rdf:resource="http://www.semanticdesktop.org/ontologies/2007/03/22/nfo#Image" />
		<rdfs:label>verticalResolution</rdfs:label>
		<rdfs:range rdf:resource="http://www.w3.org/2001/XMLSchema#integer" />
		<nrl:maxCardinality rdf:datatype="http://www.w3.org/2001/XMLSchema#integer">1</nrl:maxCardinality>
	</rdf:Property>
	<rdf:Property rdf:about="http://www.semanticdesktop.org/ontologies/2007/03/22/nfo#fileUrl">
		<nao:deprecated rdf:datatype="http://www.w3.org/2001/XMLSchema#boolean">true</nao:deprecated>
		<rdfs:comment>URL of the file. It points at the location of the file. In cases where creating a simple file:// or http:// URL for a file is difficult (e.g. for files inside compressed archives) the applications are encouraged to use conventions defined by Apache Commons VFS Project at http://jakarta.apache.org/  commons/ vfs/ filesystems.html.</rdfs:comment>
		<rdfs:domain rdf:resource="http://www.semanticdesktop.org/ontologies/2007/03/22/nfo#FileDataObject" />
		<rdfs:label>fileUrl</rdfs:label>
		<rdfs:range rdf:resource="http://www.w3.org/2000/01/rdf-schema#Resource" />
		<rdfs:subPropertyOf rdf:resource="http://www.semanticdesktop.org/ontologies/2007/01/19/nie#url" />
	</rdf:Property>
	<rdf:Property rdf:about="http://www.semanticdesktop.org/ontologies/2007/03/22/nfo#frameRate">
		<rdfs:comment>Amount of video frames per second.</rdfs:comment>
		<rdfs:domain rdf:resource="http://www.semanticdesktop.org/ontologies/2007/03/22/nfo#Video" />
		<rdfs:label>frameRate</rdfs:label>
		<rdfs:range rdf:resource="http://www.w3.org/2001/XMLSchema#float" />
		<rdfs:subPropertyOf rdf:resource="http://www.semanticdesktop.org/ontologies/2007/03/22/nfo#rate" />
		<nrl:maxCardinality rdf:datatype="http://www.w3.org/2001/XMLSchema#integer">1</nrl:maxCardinality>
	</rdf:Property>
	<rdf:Property rdf:about="http://www.semanticdesktop.org/ontologies/2007/03/22/nfo#fontFamily">
		<rdfs:comment>The name of the font family.</rdfs:comment>
		<rdfs:domain rdf:resource="http://www.semanticdesktop.org/ontologies/2007/03/22/nfo#Font" />
		<rdfs:label>fontFamily</rdfs:label>
		<rdfs:range rdf:resource="http://www.w3.org/2001/XMLSchema#string" />
		<nrl:maxCardinality rdf:datatype="http://www.w3.org/2001/XMLSchema#integer">1</nrl:maxCardinality>
	</rdf:Property>
	<rdf:Property rdf:about="http://www.semanticdesktop.org/ontologies/2007/03/22/nfo#fileCreated">
		<rdfs:comment>File creation date</rdfs:comment>
		<rdfs:domain rdf:resource="http://www.semanticdesktop.org/ontologies/2007/03/22/nfo#FileDataObject" />
		<rdfs:label>fileCreated</rdfs:label>
		<rdfs:range rdf:resource="http://www.w3.org/2001/XMLSchema#dateTime" />
		<rdfs:subPropertyOf rdf:resource="http://www.semanticdesktop.org/ontologies/2007/01/19/nie#created" />
		<nrl:maxCardinality rdf:datatype="http://www.w3.org/2001/XMLSchema#integer">1</nrl:maxCardinality>
	</rdf:Property>
	<rdf:Property rdf:about="http://www.semanticdesktop.org/ontologies/2007/03/22/nfo#bitrateType">
		<rdfs:comment>The type of the bitrate. Examples may include CBR and VBR.</rdfs:comment>
		<rdfs:domain rdf:resource="http://www.semanticdesktop.org/ontologies/2007/03/22/nfo#Media" />
		<rdfs:label>bitrateType</rdfs:label>
		<rdfs:range rdf:resource="http://www.w3.org/2001/XMLSchema#string" />
		<nrl:maxCardinality rdf:datatype="http://www.w3.org/2001/XMLSchema#integer">1</nrl:maxCardinality>
	</rdf:Property>
	<rdf:Property rdf:about="http://www.semanticdesktop.org/ontologies/2007/03/22/nfo#encoding">
		<rdfs:comment>The encoding used for the Embedded File. Examples might include BASE64 or UUEncode</rdfs:comment>
		<rdfs:domain rdf:resource="http://www.semanticdesktop.org/ontologies/2007/03/22/nfo#EmbeddedFileDataObject" />
		<rdfs:label>encoding</rdfs:label>
		<rdfs:range rdf:resource="http://www.w3.org/2001/XMLSchema#string" />
		<nrl:maxCardinality rdf:datatype="http://www.w3.org/2001/XMLSchema#integer">1</nrl:maxCardinality>
	</rdf:Property>
	<rdfs:Class rdf:about="http://www.semanticdesktop.org/ontologies/2007/03/22/nfo#Folder">
		<rdfs:comment>A folder/directory. Examples of folders include folders on a filesystem and message folders in a mailbox.</rdfs:comment>
		<rdfs:label>Folder</rdfs:label>
		<rdfs:subClassOf rdf:resource="http://www.semanticdesktop.org/ontologies/2007/03/22/nfo#DataContainer" />
	</rdfs:Class>
	<rdf:Property rdf:about="http://www.semanticdesktop.org/ontologies/2007/03/22/nfo#hasHash">
		<rdf:type rdf:resource="http://www.semanticdesktop.org/ontologies/2007/08/15/nrl#DefiningProperty" />
		<rdfs:comment>Links the file with it's hash value.</rdfs:comment>
		<rdfs:domain rdf:resource="http://www.semanticdesktop.org/ontologies/2007/03/22/nfo#FileDataObject" />
		<rdfs:label>hasHash</rdfs:label>
		<rdfs:range rdf:resource="http://www.semanticdesktop.org/ontologies/2007/03/22/nfo#FileHash" />
		<nao:userVisible rdf:datatype="http://www.w3.org/2001/XMLSchema#boolean">false</nao:userVisible>
	</rdf:Property>
	<rdf:Property rdf:about="http://www.semanticdesktop.org/ontologies/2007/03/22/nfo#codec">
		<rdfs:comment>The name of the codec necessary to decode a piece of media.</rdfs:comment>
		<rdfs:domain rdf:resource="http://www.semanticdesktop.org/ontologies/2007/03/22/nfo#Media" />
		<rdfs:label>codec</rdfs:label>
		<rdfs:range rdf:resource="http://www.w3.org/2000/01/rdf-schema#Literal" />
	</rdf:Property>
	<rdf:Property rdf:about="http://www.semanticdesktop.org/ontologies/2007/03/22/nfo#fileLastModified">
		<nao:deprecated rdf:datatype="http://www.w3.org/2001/XMLSchema#boolean">true</nao:deprecated>
		<rdfs:comment>last modification date</rdfs:comment>
		<rdfs:domain rdf:resource="http://www.semanticdesktop.org/ontologies/2007/03/22/nfo#FileDataObject" />
		<rdfs:label>fileLastModified</rdfs:label>
		<rdfs:range rdf:resource="http://www.w3.org/2001/XMLSchema#dateTime" />
		<rdfs:subPropertyOf rdf:resource="http://www.semanticdesktop.org/ontologies/2007/01/19/nie#lastModified" />
	</rdf:Property>
	<rdf:Property rdf:about="http://www.semanticdesktop.org/ontologies/2007/03/22/nfo#compressionType">
		<rdfs:comment>The type of the compression. Values include, 'lossy' and 'lossless'.</rdfs:comment>
		<rdfs:domain rdf:resource="http://www.semanticdesktop.org/ontologies/2007/03/22/nfo#Media" />
		<rdfs:label>compressionType</rdfs:label>
		<rdfs:range>
			<rdfs:Class rdf:about="http://www.semanticdesktop.org/ontologies/2007/03/22/nfo#CompressionType">
				<rdfs:comment>Type of compression. Instances of this class represent the limited set of values allowed for the nfo:compressionType property.</rdfs:comment>
				<rdfs:label>CompressionType</rdfs:label>
				<rdfs:subClassOf rdf:resource="http://www.w3.org/2000/01/rdf-schema#Resource" />
			</rdfs:Class>
		</rdfs:range>
		<nrl:maxCardinality rdf:datatype="http://www.w3.org/2001/XMLSchema#integer">1</nrl:maxCardinality>
	</rdf:Property>
	<rdf:Property rdf:about="http://www.semanticdesktop.org/ontologies/2007/03/22/nfo#pageCount">
		<rdfs:comment>Number of pages.</rdfs:comment>
		<rdfs:domain>
			<rdfs:Class rdf:about="http://www.semanticdesktop.org/ontologies/2007/03/22/nfo#PaginatedTextDocument">
				<rdfs:comment>A file containing a text document, that is unambiguously divided into pages. Examples might include PDF, DOC, PS, DVI etc.</rdfs:comment>
				<rdfs:label>PaginatedTextDocument</rdfs:label>
				<rdfs:subClassOf rdf:resource="http://www.semanticdesktop.org/ontologies/2007/03/22/nfo#TextDocument" />
			</rdfs:Class>
		</rdfs:domain>
		<rdfs:label>pageCount</rdfs:label>
		<rdfs:range rdf:resource="http://www.w3.org/2001/XMLSchema#integer" />
		<nrl:maxCardinality rdf:datatype="http://www.w3.org/2001/XMLSchema#integer">1</nrl:maxCardinality>
	</rdf:Property>
	<rdf:Property rdf:about="http://www.semanticdesktop.org/ontologies/2007/03/22/nfo#definesGlobalVariable">
		<rdfs:comment>Name of a global variable defined within the source code file.</rdfs:comment>
		<rdfs:domain rdf:resource="http://www.semanticdesktop.org/ontologies/2007/03/22/nfo#SourceCode" />
		<rdfs:label>definesGlobalVariable</rdfs:label>
		<rdfs:range rdf:resource="http://www.w3.org/2001/XMLSchema#string" />
	</rdf:Property>
	<rdfs:Class rdf:about="http://www.semanticdesktop.org/ontologies/2007/03/22/nfo#Trash">
		<rdfs:comment>Represents a container for deleted files, a feature common in modern operating systems.</rdfs:comment>
		<rdfs:label>Trash</rdfs:label>
		<rdfs:subClassOf rdf:resource="http://www.semanticdesktop.org/ontologies/2007/03/22/nfo#DataContainer" />
	</rdfs:Class>
	<rdf:Property rdf:about="http://www.semanticdesktop.org/ontologies/2007/03/22/nfo#conflicts">
		<rdfs:comment>States that a piece of software is in conflict with another piece of software.</rdfs:comment>
		<rdfs:domain rdf:resource="http://www.semanticdesktop.org/ontologies/2007/03/22/nfo#Software" />
		<rdfs:label>conflicts</rdfs:label>
		<rdfs:range rdf:resource="http://www.semanticdesktop.org/ontologies/2007/03/22/nfo#Software" />
	</rdf:Property>
	<rdf:Property rdf:about="http://www.semanticdesktop.org/ontologies/2007/03/22/nfo#encryptionStatus">
		<rdfs:comment>The status of the encryption of the InformationElement.</rdfs:comment>
		<rdfs:domain rdf:resource="http://www.semanticdesktop.org/ontologies/2007/01/19/nie#InformationElement" />
		<rdfs:label>encryptionStatus</rdfs:label>
		<rdfs:range>
			<rdfs:Class rdf:about="http://www.semanticdesktop.org/ontologies/2007/03/22/nfo#EncryptionStatus">
				<rdfs:comment>The status of the encryption of an InformationElement. nfo:encryptedStatus means that the InformationElement has been encrypted and couldn't be decrypted by the extraction software, thus no content is available. nfo:decryptedStatus means that decryption was successfull and the content is available.</rdfs:comment>
				<rdfs:label>EncryptionStatus</rdfs:label>
			</rdfs:Class>
		</rdfs:range>
		<nrl:maxCardinality rdf:datatype="http://www.w3.org/2001/XMLSchema#integer">1</nrl:maxCardinality>
	</rdf:Property>
	<rdf:Property rdf:about="http://www.semanticdesktop.org/ontologies/2007/03/22/nfo#containsBookmark">
		<rdfs:comment>The folder contains a bookmark.</rdfs:comment>
		<rdfs:domain rdf:resource="http://www.semanticdesktop.org/ontologies/2007/03/22/nfo#BookmarkFolder" />
		<rdfs:label>contains bookmark</rdfs:label>
		<rdfs:range rdf:resource="http://www.semanticdesktop.org/ontologies/2007/03/22/nfo#Bookmark" />
		<rdfs:subPropertyOf rdf:resource="http://www.semanticdesktop.org/ontologies/2007/01/19/nie#hasLogicalPart" />
	</rdf:Property>
	<rdfs:Class rdf:about="http://www.semanticdesktop.org/ontologies/2007/03/22/nfo#Executable">
		<rdfs:comment>An executable file.</rdfs:comment>
		<rdfs:label>Executable</rdfs:label>
		<rdfs:subClassOf rdf:resource="http://www.semanticdesktop.org/ontologies/2007/01/19/nie#InformationElement" />
	</rdfs:Class>
	<rdf:Property rdf:about="http://www.semanticdesktop.org/ontologies/2007/03/22/nfo#definesClass">
		<rdfs:comment>Name of a class defined in the source code file.</rdfs:comment>
		<rdfs:domain rdf:resource="http://www.semanticdesktop.org/ontologies/2007/03/22/nfo#SourceCode" />
		<rdfs:label>definesClass</rdfs:label>
		<rdfs:range rdf:resource="http://www.w3.org/2001/XMLSchema#string" />
	</rdf:Property>
	<nfo:CompressionType rdf:about="http://www.semanticdesktop.org/ontologies/2007/03/22/nfo#lossyCompressionType">
		<rdfs:label>lossyCompressionType</rdfs:label>
	</nfo:CompressionType>
	<rdfs:Class rdf:about="http://www.semanticdesktop.org/ontologies/2007/03/22/nfo#OperatingSystem">
		<rdfs:comment>An OperatingSystem</rdfs:comment>
		<rdfs:label>OperatingSystem</rdfs:label>
		<rdfs:subClassOf rdf:resource="http://www.semanticdesktop.org/ontologies/2007/03/22/nfo#Software" />
	</rdfs:Class>
	<rdf:Property rdf:about="http://www.semanticdesktop.org/ontologies/2007/03/22/nfo#fileSize">
		<rdfs:comment>The size of the file in bytes. For compressed files it means the size of the packed file, not of the contents. For folders it means the aggregated size of all contained files and folders </rdfs:comment>
		<rdfs:domain rdf:resource="http://www.semanticdesktop.org/ontologies/2007/03/22/nfo#FileDataObject" />
		<rdfs:label>fileSize</rdfs:label>
		<rdfs:range rdf:resource="http://www.w3.org/2001/XMLSchema#integer" />
		<rdfs:subPropertyOf rdf:resource="http://www.semanticdesktop.org/ontologies/2007/01/19/nie#byteSize" />
		<nrl:maxCardinality rdf:datatype="http://www.w3.org/2001/XMLSchema#integer">1</nrl:maxCardinality>
	</rdf:Property>
	<rdfs:Class rdf:about="http://www.semanticdesktop.org/ontologies/2007/03/22/nfo#RemoteDataObject">
		<rdfs:comment>A file data object stored at a remote location. Don't confuse this class with a RemotePortAddress. This one applies to a particular resource, RemotePortAddress applies to an address, that can have various interpretations.</rdfs:comment>
		<rdfs:label>RemoteDataObject</rdfs:label>
		<rdfs:subClassOf rdf:resource="http://www.semanticdesktop.org/ontologies/2007/03/22/nfo#FileDataObject" />
	</rdfs:Class>
	<rdf:Property rdf:about="http://www.semanticdesktop.org/ontologies/2007/03/22/nfo#colorCount">
		<rdfs:label>color count</rdfs:label>
		<rdfs:comment>The number of colors used/available in a raster image.</rdfs:comment>
		<rdfs:domain rdf:resource="http://www.semanticdesktop.org/ontologies/2007/03/22/nfo#RasterImage" />
		<rdfs:range rdf:resource="http://www.w3.org/2001/XMLSchema#integer" />
		<nrl:maxCardinality rdf:datatype="http://www.w3.org/2001/XMLSchema#integer">1</nrl:maxCardinality>
	</rdf:Property>
	<rdf:Property rdf:about="http://www.semanticdesktop.org/ontologies/2007/03/22/nfo#paletteSize">
		<rdfs:label>palette size</rdfs:label>
		<rdfs:comment>The number of colors defined in palette of the raster image.</rdfs:comment>
		<rdfs:domain rdf:resource="http://www.semanticdesktop.org/ontologies/2007/03/22/nfo#RasterImage" />
		<rdfs:range rdf:resource="http://www.w3.org/2001/XMLSchema#integer" />
		<nrl:maxCardinality rdf:datatype="http://www.w3.org/2001/XMLSchema#integer">1</nrl:maxCardinality>
	</rdf:Property>
	<rdfs:Class rdf:about="http://www.semanticdesktop.org/ontologies/2007/03/22/nfo#WebDataObject">
		<rdfs:subClassOf rdf:resource="http://www.semanticdesktop.org/ontologies/2007/01/19/nie#DataObject" />
		<rdfs:label>web data object</rdfs:label>
		<rdfs:comment>An information resources of which representations (files, streams) can be retrieved through a web server. They may be generated at retrieval time. Typical examples are pages served by PHP or AJAX or mp3 streams.</rdfs:comment>
	</rdfs:Class>
	<rdfs:Class rdf:about="http://www.semanticdesktop.org/ontologies/2007/03/22/nfo#LocalFileDataObject">
		<rdfs:subClassOf rdf:resource="http://www.semanticdesktop.org/ontologies/2007/03/22/nfo#FileDataObject" />
		<rdfs:label>local file</rdfs:label>
		<rdfs:comment>A local file data object which is stored on a local file system. Its nie:url always uses the file:/ protocol. The main use of this class is to distinguish local and non-local files.</rdfs:comment>
	</rdfs:Class>
	<rdf:Property rdf:about="http://www.semanticdesktop.org/ontologies/2007/03/22/nfo#depiction">
		<rdfs:comment>Relates an information element to an image which depicts said element.</rdfs:comment>
		<rdfs:domain rdf:resource="http://www.w3.org/2000/01/rdf-schema#Resource" />
		<rdfs:label>depiction</rdfs:label>
		<rdfs:range rdf:resource="http://www.semanticdesktop.org/ontologies/2007/03/22/nfo#Image" />
		<nrl:inverseProperty>
			<rdf:Property rdf:about="http://www.semanticdesktop.org/ontologies/2007/03/22/nfo#depicts">
				<rdfs:comment>Relates an image to the information elements it depicts.</rdfs:comment>
				<rdfs:domain rdf:resource="http://www.semanticdesktop.org/ontologies/2007/03/22/nfo#Image" />
				<rdfs:label>depicts</rdfs:label>
				<rdfs:range rdf:resource="http://www.w3.org/2000/01/rdf-schema#Resource" />
				<nrl:inverseProperty rdf:resource="http://www.semanticdesktop.org/ontologies/2007/03/22/nfo#depiction" />
			</rdf:Property>
		</nrl:inverseProperty>
	</rdf:Property>
	<rdf:Property rdf:about="http://www.semanticdesktop.org/ontologies/2007/03/22/nfo#containsPlacemark">
		<rdfs:comment>Containment relation between placemark containers (files) and placemarks within.</rdfs:comment>
		<rdfs:domain>
			<rdfs:Class rdf:about="http://www.semanticdesktop.org/ontologies/2007/03/22/nfo#PlacemarkContainer">
				<rdfs:comment>A data object containing placemark(s). Use nie:contentCreated to represent the date when the user created the dataobject, nao:creator for defining the creator, nie:contentLastModified for modifications. nfo:containsPlacemark to refer to individual placemarks within.</rdfs:comment>
				<rdfs:label>Placemark Container</rdfs:label>
				<rdfs:subClassOf rdf:resource="http://www.semanticdesktop.org/ontologies/2007/01/19/nie#InformationElement" />
			</rdfs:Class>
		</rdfs:domain>
		<rdfs:label>contains Placemark</rdfs:label>
		<rdfs:range>
			<rdfs:Class rdf:about="http://www.semanticdesktop.org/ontologies/2007/03/22/nfo#Placemark">
				<rdfs:comment>One placemark within a placemark container/file. Use nie:title for the name/label, nao:creator for defining the creator.</rdfs:comment>
				<rdfs:label>Placemark</rdfs:label>
				<rdfs:subClassOf rdf:resource="http://www.semanticdesktop.org/ontologies/2007/01/19/nie#InformationElement" />
			</rdfs:Class>
		</rdfs:range>
		<rdfs:subPropertyOf rdf:resource="http://www.semanticdesktop.org/ontologies/2007/01/19/nie#hasLogicalPart" />
	</rdf:Property>
</rdf:RDF>