<?xml version="1.0" encoding="utf-8" ?>
<rdf:RDF xmlns:rdf="http://www.w3.org/1999/02/22-rdf-syntax-ns#"
         xmlns:owl="http://www.w3.org/2002/07/owl#"
         xmlns:dc="http://purl.org/dc/terms/"
         xmlns:rdfs="http://www.w3.org/2000/01/rdf-schema#"
         xmlns:skos="http://www.w3.org/2004/02/skos/core#">

  <owl:Ontology rdf:about="http://w3id.org/art/terms/1.0/">
    <dc:title xml:lang="en">Artivity Ontology, Version 1.0</dc:title>
    <dc:modified rdf:datatype="http://www.w3.org/2001/XMLSchema#date">2016-06-06</dc:modified>
    <dc:publisher rdf:resource="http://artivity.io/about"/>
  </owl:Ontology>

  <rdf:Description rdf:about="http://www.semanticdesktop.org/ontologies/2007/03/22/nfo#VectorImage">
    <rdfs:subClassOf rdf:resource="http://www.w3.org/ns/prov#Entity"/>
  </rdf:Description>

  <rdf:Description rdf:about="http://www.semanticdesktop.org/ontologies/2007/03/22/nfo#RasterImage">
    <rdfs:subClassOf rdf:resource="http://www.w3.org/ns/prov#Entity"/>
  </rdf:Description>

  <rdf:Description rdf:about="http://www.semanticdesktop.org/ontologies/2007/03/22/nfo#Website">
    <rdfs:subClassOf rdf:resource="http://www.w3.org/ns/prov#Entity"/>
  </rdf:Description>

  <rdfs:Class rdf:about="http://w3id.org/art/terms/1.0/BoundingRectangle">
    <rdfs:subClassOf rdf:resource="http://w3id.org/art/terms/1.0/Rectangle"/>
    <rdfs:label xml:lang="en">BoundingRectangle</rdfs:label>
    <rdfs:comment xml:lang="en">An expression of the maximum extents of a 2-dimensional object (e.g. point, line, polygon) or set of objects within their 2-D coordinate system. In other words min(x), max(x), min(y), max(y).</rdfs:comment>
    <rdfs:isDefinedBy rdf:resource="http://w3id.org/art/terms/1.0/"/>
    <rdfs:seeAlso rdf:resource="https://en.wikipedia.org/wiki/Minimum_bounding_rectangle"/>
    <dc:issued rdf:datatype="http://www.w3.org/2001/XMLSchema#date">2016-06-06</dc:issued>
    <dc:modified rdf:datatype="http://www.w3.org/2001/XMLSchema#date">2016-06-06</dc:modified>
  </rdfs:Class>

  <rdfs:Class rdf:about="http://w3id.org/art/terms/1.0/Canvas">
    <rdfs:subClassOf rdf:resource="http://w3id.org/art/terms/1.0/Rectangle"/>
    <rdfs:label xml:lang="en">Canvas</rdfs:label>
    <rdfs:comment xml:lang="en">An entity that defines the 2-dimensional extents of the printable or renderable region(s) of a document.</rdfs:comment>
    <rdfs:isDefinedBy rdf:resource="http://w3id.org/art/terms/1.0/"/>
    <dc:issued rdf:datatype="http://www.w3.org/2001/XMLSchema#date">2016-06-06</dc:issued>
    <dc:modified rdf:datatype="http://www.w3.org/2001/XMLSchema#date">2016-06-06</dc:modified>
  </rdfs:Class>

  <rdfs:Class rdf:about="http://w3id.org/art/terms/1.0/CartesianCoordinateSystem">
    <rdfs:subClassOf rdf:resource="http://w3id.org/art/terms/1.0/CoordinateSystem"/>
    <rdfs:label xml:lang="en">CartesianCoordinateSystem</rdfs:label>
    <rdfs:comment xml:lang="en">A coordinate system that specifies each point uniquely using n Cartesian coordinates which specify the point in an n-dimensional Euclidean space for any dimension n. These coordinates are equal, up to sign, to distances from the point to n mutually perpendicular hyperplanes.</rdfs:comment>
    <rdfs:isDefinedBy rdf:resource="http://w3id.org/art/terms/1.0/"/>
    <rdfs:seeAlso rdf:resource="https://en.wikipedia.org/wiki/Cartesian_coordinate_system"/>
    <dc:issued rdf:datatype="http://www.w3.org/2001/XMLSchema#date">2016-06-06</dc:issued>
    <dc:modified rdf:datatype="http://www.w3.org/2001/XMLSchema#date">2016-06-06</dc:modified>
  </rdfs:Class>

  <rdfs:Class rdf:about="http://w3id.org/art/terms/1.0/CoordinateSystem">
    <rdfs:label xml:lang="en">CoordinateSystem</rdfs:label>
    <rdfs:comment xml:lang="en">A system which uses one or more numbers (coordinates) to uniquely determine the position of a point or other geometric element on a manifold such as Euclidean space.</rdfs:comment>
    <rdfs:isDefinedBy rdf:resource="http://w3id.org/art/terms/1.0/"/>
    <rdfs:seeAlso rdf:resource="https://en.wikipedia.org/wiki/Coordinate_system"/>
    <dc:issued rdf:datatype="http://www.w3.org/2001/XMLSchema#date">2016-06-06</dc:issued>
    <dc:modified rdf:datatype="http://www.w3.org/2001/XMLSchema#date">2016-06-06</dc:modified>
  </rdfs:Class>

  <rdfs:Class rdf:about="http://w3id.org/art/terms/1.0/CreateFile">
    <rdfs:subClassOf rdf:resource="http://www.w3.org/ns/prov#Activity"/>
    <rdfs:label xml:lang="en">CreateFile</rdfs:label>
    <rdfs:comment xml:lang="en">An activity which resulted in a new file being generated.</rdfs:comment>
    <rdfs:isDefinedBy rdf:resource="http://w3id.org/art/terms/1.0/"/>
    <dc:issued rdf:datatype="http://www.w3.org/2001/XMLSchema#date">2016-06-06</dc:issued>
    <dc:modified rdf:datatype="http://www.w3.org/2001/XMLSchema#date">2016-06-06</dc:modified>
  </rdfs:Class>

  <rdfs:Class rdf:about="http://w3id.org/art/terms/1.0/EditFile">
    <rdfs:subClassOf rdf:resource="http://www.w3.org/ns/prov#Activity"/>
    <rdfs:label xml:lang="en">EditFile</rdfs:label>
    <rdfs:comment xml:lang="en">An activity which may result in an existing file being revised and/or modified.</rdfs:comment>
    <rdfs:isDefinedBy rdf:resource="http://w3id.org/art/terms/1.0/"/>
    <dc:issued rdf:datatype="http://www.w3.org/2001/XMLSchema#date">2016-06-06</dc:issued>
    <dc:modified rdf:datatype="http://www.w3.org/2001/XMLSchema#date">2016-06-06</dc:modified>
  </rdfs:Class>

  <rdfs:Class rdf:about="http://w3id.org/art/terms/1.0/DeleteFile">
    <rdfs:subClassOf rdf:resource="http://www.w3.org/ns/prov#Activity"/>
    <rdfs:label xml:lang="en">DeleteFile</rdfs:label>
    <rdfs:comment xml:lang="en">An activity which resulted in an existing file being deleted.</rdfs:comment>
    <rdfs:isDefinedBy rdf:resource="http://w3id.org/art/terms/1.0/"/>
    <dc:issued rdf:datatype="http://www.w3.org/2001/XMLSchema#date">2016-06-06</dc:issued>
    <dc:modified rdf:datatype="http://www.w3.org/2001/XMLSchema#date">2016-06-06</dc:modified>
  </rdfs:Class>

  <rdfs:Class rdf:about="http://w3id.org/art/terms/1.0/EntityGroup">
    <rdfs:subClassOf rdf:resource="http://www.w3.org/ns/prov#Entity"/>
    <rdfs:label xml:lang="en">EntityGroup</rdfs:label>
    <rdfs:comment xml:lang="en">A set of entities.</rdfs:comment>
    <rdfs:isDefinedBy rdf:resource="http://w3id.org/art/terms/1.0/"/>
    <dc:issued rdf:datatype="http://www.w3.org/2001/XMLSchema#date">2016-06-06</dc:issued>
    <dc:modified rdf:datatype="http://www.w3.org/2001/XMLSchema#date">2016-06-06</dc:modified>
  </rdfs:Class>

  <rdfs:Class rdf:about="http://w3id.org/art/terms/1.0/Layer">
    <rdfs:subClassOf rdf:resource="http://www.w3.org/ns/prov#Entity"/>
    <rdfs:label xml:lang="en">Layer</rdfs:label>
    <rdfs:comment xml:lang="en">Establishes a depth hierarchy amongst separate entities of a 2-dimensional digital image.</rdfs:comment>
    <rdfs:isDefinedBy rdf:resource="http://w3id.org/art/terms/1.0/"/>
    <dc:issued rdf:datatype="http://www.w3.org/2001/XMLSchema#date">2016-06-06</dc:issued>
    <dc:modified rdf:datatype="http://www.w3.org/2001/XMLSchema#date">2016-06-06</dc:modified>
  </rdfs:Class>

  <rdfs:Class rdf:about="http://w3id.org/art/terms/1.0/LengthUnit">
    <rdfs:label xml:lang="en">LengthUnit</rdfs:label>
    <rdfs:comment xml:lang="en">Refers to any discrete, pre-established length or distance having a constant magnitude which is used as a reference or convention to express linear dimension.</rdfs:comment>
    <rdfs:isDefinedBy rdf:resource="http://w3id.org/art/terms/1.0/"/>
    <dc:issued rdf:datatype="http://www.w3.org/2001/XMLSchema#date">2016-06-06</dc:issued>
    <dc:modified rdf:datatype="http://www.w3.org/2001/XMLSchema#date">2016-06-06</dc:modified>
  </rdfs:Class>

  <rdfs:Class rdf:about="http://w3id.org/art/terms/1.0/PartialRenderingDataObject">
    <rdfs:subClassOf>
      <rdfs:Class rdf:about="http://w3id.org/art/terms/1.0/RenderingDataObject">
        <rdfs:subClassOf rdf:resource="http://www.semanticdesktop.org/ontologies/2007/03/22/nfo#FileDataObject"/>
        <rdfs:label xml:lang="en">RenderingDataObject</rdfs:label>
        <rdfs:comment xml:lang="en">Rasterized bitmap data of the entire extents of an image.</rdfs:comment>
        <rdfs:isDefinedBy rdf:resource="http://w3id.org/art/terms/1.0/"/>
        <dc:issued rdf:datatype="http://www.w3.org/2001/XMLSchema#date">2016-06-06</dc:issued>
        <dc:modified rdf:datatype="http://www.w3.org/2001/XMLSchema#date">2016-06-06</dc:modified>
      </rdfs:Class>
    </rdfs:subClassOf>

    <rdfs:label xml:lang="en">PartialRenderingDataObject</rdfs:label>
    <rdfs:comment xml:lang="en">Rasterized bitmap data of a specific region of an image.</rdfs:comment>
    <rdfs:isDefinedBy rdf:resource="http://w3id.org/art/terms/1.0/"/>
    <dc:issued rdf:datatype="http://www.w3.org/2001/XMLSchema#date">2016-06-06</dc:issued>
    <dc:modified rdf:datatype="http://www.w3.org/2001/XMLSchema#date">2016-06-06</dc:modified>
  </rdfs:Class>

  <rdfs:Class rdf:about="http://w3id.org/art/terms/1.0/Point">
    <rdfs:subClassOf rdf:resource="http://www.opengis.net/ont/geosparql#SpatialObject"/>
    <rdfs:label xml:lang="en">Point</rdfs:label>
    <rdfs:comment xml:lang="en">An entity that captures the notion of a unique location in Euclidean space.</rdfs:comment>
    <rdfs:isDefinedBy rdf:resource="http://w3id.org/art/terms/1.0/"/>
    <rdfs:seeAlso rdf:resource="https://en.wikipedia.org/wiki/Point_(geometry)"/>
    <dc:issued rdf:datatype="http://www.w3.org/2001/XMLSchema#date">2016-06-06</dc:issued>
    <dc:modified rdf:datatype="http://www.w3.org/2001/XMLSchema#date">2016-06-06</dc:modified>
  </rdfs:Class>

  <rdfs:Class rdf:about="http://w3id.org/art/terms/1.0/Rectangle">
    <rdfs:subClassOf rdf:resource="http://www.w3.org/ns/prov#Entity"/>
    <rdfs:subClassOf rdf:resource="http://www.opengis.net/ont/geosparql#Geometry"/>
    <rdfs:label xml:lang="en">Rectangle</rdfs:label>
    <rdfs:comment xml:lang="en">A parallelogram containing a right angle.</rdfs:comment>
    <rdfs:isDefinedBy rdf:resource="http://w3id.org/art/terms/1.0/"/>
    <rdfs:seeAlso rdf:resource="https://en.wikipedia.org/wiki/Rectangle"/>
    <dc:issued rdf:datatype="http://www.w3.org/2001/XMLSchema#date">2016-06-06</dc:issued>
    <dc:modified rdf:datatype="http://www.w3.org/2001/XMLSchema#date">2016-06-06</dc:modified>
  </rdfs:Class>

  <rdfs:Class rdf:about="http://w3id.org/art/terms/1.0/Redo">
    <rdfs:subClassOf rdf:resource="http://www.w3.org/ns/prov#EntityInfluence"/>
    <rdfs:label xml:lang="en">Redo</rdfs:label>
    <rdfs:comment xml:lang="en">The re-generation of a formerly undone entity influence.</rdfs:comment>
    <rdfs:isDefinedBy rdf:resource="http://w3id.org/art/terms/1.0/"/>
    <dc:issued rdf:datatype="http://www.w3.org/2001/XMLSchema#date">2016-06-06</dc:issued>
    <dc:modified rdf:datatype="http://www.w3.org/2001/XMLSchema#date">2016-06-06</dc:modified>
  </rdfs:Class>

  <rdfs:Class rdf:about="http://w3id.org/art/terms/1.0/Undo">
    <rdfs:subClassOf rdf:resource="http://www.w3.org/ns/prov#EntityInfluence"/>
    <rdfs:label xml:lang="en">Undo</rdfs:label>
    <rdfs:comment xml:lang="en">The invalidation of an existing entity influence.</rdfs:comment>
    <rdfs:isDefinedBy rdf:resource="http://w3id.org/art/terms/1.0/"/>
    <dc:issued rdf:datatype="http://www.w3.org/2001/XMLSchema#date">2016-06-06</dc:issued>
    <dc:modified rdf:datatype="http://www.w3.org/2001/XMLSchema#date">2016-06-06</dc:modified>
  </rdfs:Class>

  <rdfs:Class rdf:about="http://w3id.org/art/terms/1.0/ViewFile">
    <rdfs:subClassOf rdf:resource="http://www.w3.org/ns/prov#Activity"/>
    <rdfs:label xml:lang="en">ViewFile</rdfs:label>
    <rdfs:comment xml:lang="en">An activity in which a file was viewed by one or more users.</rdfs:comment>
    <rdfs:isDefinedBy rdf:resource="http://w3id.org/art/terms/1.0/"/>
    <dc:issued rdf:datatype="http://www.w3.org/2001/XMLSchema#date">2016-06-06</dc:issued>
    <dc:modified rdf:datatype="http://www.w3.org/2001/XMLSchema#date">2016-06-06</dc:modified>
  </rdfs:Class>

  <rdfs:Class rdf:about="http://w3id.org/art/terms/1.0/Viewport">
    <rdfs:subClassOf rdf:resource="http://w3id.org/art/terms/1.0/Rectangle"/>
    <rdfs:label xml:lang="en">Viewport</rdfs:label>
    <rdfs:comment xml:lang="en">A rectangle that represents the visible portion of a document.</rdfs:comment>
    <rdfs:isDefinedBy rdf:resource="http://w3id.org/art/terms/1.0/"/>
    <rdfs:seeAlso rdf:resource="https://en.wikipedia.org/wiki/Viewport"/>
    <dc:issued rdf:datatype="http://www.w3.org/2001/XMLSchema#date">2016-06-06</dc:issued>
    <dc:modified rdf:datatype="http://www.w3.org/2001/XMLSchema#date">2016-06-06</dc:modified>
  </rdfs:Class>

  <rdfs:Class rdf:about="http://w3id.org/art/terms/1.0/WebBrowsing">
    <rdfs:subClassOf rdf:resource="http://www.w3.org/ns/prov#Activity"/>
    <rdfs:label xml:lang="en">WebBrowsing</rdfs:label>
    <rdfs:comment xml:lang="en">An activity in which one or more websites were viewed by one or more users.</rdfs:comment>
    <rdfs:isDefinedBy rdf:resource="http://w3id.org/art/terms/1.0/"/>
    <dc:issued rdf:datatype="http://www.w3.org/2001/XMLSchema#date">2016-06-06</dc:issued>
    <dc:modified rdf:datatype="http://www.w3.org/2001/XMLSchema#date">2016-06-06</dc:modified>
  </rdfs:Class>

  <rdf:Property rdf:about="http://w3id.org/art/terms/1.0/aboveLayer">
    <rdfs:label xml:lang="en">aboveLayer</rdfs:label>
    <rdfs:comment xml:lang="en">Indicates that the contents of a layer are placed on top of the referenced layer.</rdfs:comment>
    <rdfs:isDefinedBy rdf:resource="http://w3id.org/art/terms/1.0/"/>
    <rdfs:domain rdf:resource="http://w3id.org/art/terms/1.0/Layer"/>
    <rdfs:range rdf:resource="http://w3id.org/art/terms/1.0/Layer"/>
    <dc:issued rdf:datatype="http://www.w3.org/2001/XMLSchema#date">2016-06-06</dc:issued>
    <dc:modified rdf:datatype="http://www.w3.org/2001/XMLSchema#date">2016-06-06</dc:modified>
  </rdf:Property>

  <rdf:Property rdf:about="http://w3id.org/art/terms/1.0/boundaries">
    <rdfs:label xml:lang="en">boundaries</rdfs:label>
    <rdfs:comment xml:lang="en">References a geometry that provides the minimum bounds for a geometry or group of geometries.</rdfs:comment>
    <rdfs:isDefinedBy rdf:resource="http://w3id.org/art/terms/1.0/"/>
    <rdfs:domain rdf:resource="http://www.w3.org/ns/prov#Entity"/>
    <rdfs:domain rdf:resource="http://www.w3.org/ns/prov#EntityInfluence"/>
    <rdfs:range rdf:resource="http://w3id.org/art/terms/1.0/BoundingRectangle"/>
    <dc:issued rdf:datatype="http://www.w3.org/2001/XMLSchema#date">2016-06-06</dc:issued>
    <dc:modified rdf:datatype="http://www.w3.org/2001/XMLSchema#date">2016-06-06</dc:modified>
  </rdf:Property>

  <rdf:Property rdf:about="http://w3id.org/art/terms/1.0/canvas">
    <rdfs:label xml:lang="en">canvas</rdfs:label>
    <rdfs:comment xml:lang="en">References a rectangle that defines the printable or renderable region of a document.</rdfs:comment>
    <rdfs:isDefinedBy rdf:resource="http://w3id.org/art/terms/1.0/"/>
    <rdfs:domain rdf:resource="http://www.semanticdesktop.org/ontologies/2007/03/22/nfo#VectorImage"/>
    <rdfs:domain rdf:resource="http://www.semanticdesktop.org/ontologies/2007/03/22/nfo#RasterImage"/>
    <rdfs:range rdf:resource="http://w3id.org/art/terms/1.0/Canvas"/>
    <dc:issued rdf:datatype="http://www.w3.org/2001/XMLSchema#date">2016-06-06</dc:issued>
    <dc:modified rdf:datatype="http://www.w3.org/2001/XMLSchema#date">2016-06-06</dc:modified>
  </rdf:Property>

  <rdf:Property rdf:about="http://w3id.org/art/terms/1.0/colorCode">
    <rdfs:label xml:lang="en">colorCode</rdfs:label>
    <rdfs:comment xml:lang="en">An associated color encoded in a RGB or ARGB hex string.</rdfs:comment>
    <rdfs:isDefinedBy rdf:resource="http://w3id.org/art/terms/1.0/"/>
    <rdfs:seeAlso rdf:resource="https://en.wikipedia.org/wiki/Web_colors#Hex_triplet"/>
    <rdfs:domain rdf:resource="http://www.w3.org/ns/prov#Entity"/>
    <rdfs:range rdf:resource="http://www.w3.org/2001/XMLSchema#string"/>
    <dc:issued rdf:datatype="http://www.w3.org/2001/XMLSchema#date">2016-06-06</dc:issued>
    <dc:modified rdf:datatype="http://www.w3.org/2001/XMLSchema#date">2016-06-06</dc:modified>
  </rdf:Property>

  <rdf:Property rdf:about="http://w3id.org/art/terms/1.0/coordinateDimension">
    <rdfs:label xml:lang="en">coordinateDimension</rdfs:label>
    <rdfs:comment xml:lang="en">The number of coordinates that are required to uniquely identify a position in a coordinate system.</rdfs:comment>
    <rdfs:isDefinedBy rdf:resource="http://w3id.org/art/terms/1.0/"/>
    <rdfs:domain rdf:resource="http://w3id.org/art/terms/1.0/CoordinateSystem"/>
    <rdfs:range rdf:resource="http://www.w3.org/2001/XMLSchema#integer"/>
    <dc:issued rdf:datatype="http://www.w3.org/2001/XMLSchema#date">2016-06-06</dc:issued>
    <dc:modified rdf:datatype="http://www.w3.org/2001/XMLSchema#date">2016-06-06</dc:modified>
  </rdf:Property>

  <rdf:Property rdf:about="http://w3id.org/art/terms/1.0/coordinateSystem">
    <rdfs:label xml:lang="en">coordinateSystem</rdfs:label>
    <rdfs:comment xml:lang="en">The coordinate system that is used to locate geometries in a document.</rdfs:comment>
    <rdfs:isDefinedBy rdf:resource="http://w3id.org/art/terms/1.0/"/>
    <rdfs:domain rdf:resource="http://www.semanticdesktop.org/ontologies/2007/03/22/nfo#VectorImage"/>
    <rdfs:domain rdf:resource="http://www.semanticdesktop.org/ontologies/2007/03/22/nfo#RasterImage"/>
    <rdfs:range rdf:resource="http://w3id.org/art/terms/1.0/CoordinateSystem"/>
    <dc:issued rdf:datatype="http://www.w3.org/2001/XMLSchema#date">2016-06-06</dc:issued>
    <dc:modified rdf:datatype="http://www.w3.org/2001/XMLSchema#date">2016-06-06</dc:modified>
  </rdf:Property>

  <rdf:Property rdf:about="http://w3id.org/art/terms/1.0/depth">
    <rdfs:label xml:lang="en">depth</rdfs:label>
    <rdfs:comment xml:lang="en">The extents of a geometry along the z-axis of a Cartesian coordinate system.</rdfs:comment>
    <rdfs:isDefinedBy rdf:resource="http://w3id.org/art/terms/1.0/"/>
    <rdfs:domain rdf:resource="http://www.opengis.net/ont/geosparql#Geometry"/>
    <rdfs:range rdf:resource="http://www.w3.org/2001/XMLSchema#double"/>
    <dc:issued rdf:datatype="http://www.w3.org/2001/XMLSchema#date">2016-06-06</dc:issued>
    <dc:modified rdf:datatype="http://www.w3.org/2001/XMLSchema#date">2016-06-06</dc:modified>
  </rdf:Property>

  <rdf:Property rdf:about="http://w3id.org/art/terms/1.0/executable">
    <rdfs:label xml:lang="en">executable</rdfs:label>
    <rdfs:comment xml:lang="en">The executable program file data object of a software agent.</rdfs:comment>
    <rdfs:isDefinedBy rdf:resource="http://w3id.org/art/terms/1.0/"/>
    <rdfs:domain rdf:resource="http://www.w3.org/ns/prov#SoftwareAgent"/>
    <rdfs:range rdf:resource="http://www.semanticdesktop.org/ontologies/2007/03/22/nfo#FileDataObject"/>
    <dc:issued rdf:datatype="http://www.w3.org/2001/XMLSchema#date">2016-06-06</dc:issued>
    <dc:modified rdf:datatype="http://www.w3.org/2001/XMLSchema#date">2016-06-06</dc:modified>
  </rdf:Property>

  <rdf:Property rdf:about="http://w3id.org/art/terms/1.0/group">
    <rdfs:label xml:lang="en">group</rdfs:label>
    <rdfs:comment xml:lang="en">Establishes a part-of relationship between an entity a group of entities.</rdfs:comment>
    <rdfs:isDefinedBy rdf:resource="http://w3id.org/art/terms/1.0/"/>
    <rdfs:domain rdf:resource="http://www.w3.org/ns/prov#Entity"/>
    <rdfs:range rdf:resource="http://w3id.org/art/terms/1.0/EntityGroup"/>
    <dc:issued rdf:datatype="http://www.w3.org/2001/XMLSchema#date">2016-06-06</dc:issued>
    <dc:modified rdf:datatype="http://www.w3.org/2001/XMLSchema#date">2016-06-06</dc:modified>
  </rdf:Property>

  <rdf:Property rdf:about="http://w3id.org/art/terms/1.0/height">
    <rdfs:label xml:lang="en">height</rdfs:label>
    <rdfs:comment xml:lang="en">The extents of a geometry along the y-axis of a Cartesian coordinate system.</rdfs:comment>
    <rdfs:isDefinedBy rdf:resource="http://w3id.org/art/terms/1.0/"/>
    <rdfs:domain rdf:resource="http://www.opengis.net/ont/geosparql#Geometry"/>
    <rdfs:range rdf:resource="http://www.w3.org/2001/XMLSchema#double"/>
    <dc:issued rdf:datatype="http://www.w3.org/2001/XMLSchema#date">2016-06-06</dc:issued>
    <dc:modified rdf:datatype="http://www.w3.org/2001/XMLSchema#date">2016-06-06</dc:modified>
  </rdf:Property>

  <rdf:Property rdf:about="http://w3id.org/art/terms/1.0/layer">
    <rdfs:label xml:lang="en">layer</rdfs:label>
    <rdfs:comment xml:lang="en">Establishes a relationship between an object an a layer.</rdfs:comment>
    <rdfs:isDefinedBy rdf:resource="http://w3id.org/art/terms/1.0/"/>
    <rdfs:domain rdf:resource="http://www.w3.org/ns/prov#Entity"/>
    <rdfs:range rdf:resource="http://w3id.org/art/terms/1.0/Layer"/>
    <dc:issued rdf:datatype="http://www.w3.org/2001/XMLSchema#date">2016-06-06</dc:issued>
    <dc:modified rdf:datatype="http://www.w3.org/2001/XMLSchema#date">2016-06-06</dc:modified>
  </rdf:Property>

  <rdf:Property rdf:about="http://w3id.org/art/terms/1.0/lengthUnit">
    <rdfs:label xml:lang="en">lengthUnit</rdfs:label>
    <rdfs:comment xml:lang="en">Specifies the length unit used for the coordinates in a coordinate system.</rdfs:comment>
    <rdfs:isDefinedBy rdf:resource="http://w3id.org/art/terms/1.0/"/>
    <rdfs:domain rdf:resource="http://w3id.org/art/terms/1.0/CoordinateSystem"/>
    <rdfs:range rdf:resource="http://w3id.org/art/terms/1.0/LengthUnit"/>
    <dc:issued rdf:datatype="http://www.w3.org/2001/XMLSchema#date">2016-06-06</dc:issued>
    <dc:modified rdf:datatype="http://www.w3.org/2001/XMLSchema#date">2016-06-06</dc:modified>
  </rdf:Property>

  <rdf:Property rdf:about="http://w3id.org/art/terms/1.0/loggingEnabled">
    <rdfs:label xml:lang="en">loggingEnabled</rdfs:label>
    <rdfs:comment xml:lang="en">Indicates if the logging of activities is enabled for a software agent.</rdfs:comment>
    <rdfs:isDefinedBy rdf:resource="http://w3id.org/art/terms/1.0/"/>
    <rdfs:domain rdf:resource="http://www.w3.org/ns/prov#SoftwareAgent"/>
    <rdfs:range rdf:resource="http://www.w3.org/2001/XMLSchema#boolean"/>
    <dc:issued rdf:datatype="http://www.w3.org/2001/XMLSchema#date">2016-06-06</dc:issued>
    <dc:modified rdf:datatype="http://www.w3.org/2001/XMLSchema#date">2016-06-06</dc:modified>
  </rdf:Property>

  <rdf:Property rdf:about="http://w3id.org/art/terms/1.0/parentLayer">
    <rdfs:label xml:lang="en">parentLayer</rdfs:label>
    <rdfs:comment xml:lang="en">Indicates that a layer is logically contained in the referenced layer.</rdfs:comment>
    <rdfs:isDefinedBy rdf:resource="http://w3id.org/art/terms/1.0/"/>
    <rdfs:domain rdf:resource="http://w3id.org/art/terms/1.0/Layer"/>
    <rdfs:range rdf:resource="http://w3id.org/art/terms/1.0/Layer"/>
    <dc:issued rdf:datatype="http://www.w3.org/2001/XMLSchema#date">2016-06-06</dc:issued>
    <dc:modified rdf:datatype="http://www.w3.org/2001/XMLSchema#date">2016-06-06</dc:modified>
  </rdf:Property>

  <rdf:Property rdf:about="http://w3id.org/art/terms/1.0/pluginFolder">
    <rdfs:label xml:lang="en">pluginFolder</rdfs:label>
    <rdfs:comment xml:lang="en">The file system folder containing the program extension (plugin) of the Artivity software agent.</rdfs:comment>
    <rdfs:isDefinedBy rdf:resource="http://w3id.org/art/terms/1.0/"/>
    <rdfs:domain rdf:resource="http://www.w3.org/ns/prov#SoftwareAgent"/>
    <rdfs:range rdf:resource="http://www.semanticdesktop.org/ontologies/2007/03/22/nfo#Folder"/>
    <dc:issued rdf:datatype="http://www.w3.org/2001/XMLSchema#date">2016-06-06</dc:issued>
    <dc:modified rdf:datatype="http://www.w3.org/2001/XMLSchema#date">2016-06-06</dc:modified>
  </rdf:Property>

  <rdf:Property rdf:about="http://w3id.org/art/terms/1.0/position">
    <rdfs:label xml:lang="en">position</rdfs:label>
    <rdfs:comment xml:lang="en">Location of a geometry in Euclidean space.</rdfs:comment>
    <rdfs:isDefinedBy rdf:resource="http://w3id.org/art/terms/1.0/"/>
    <rdfs:domain rdf:resource="http://www.opengis.net/ont/geosparql#Geometry"/>
    <rdfs:range rdf:resource="http://w3id.org/art/terms/1.0/Point"/>
    <dc:issued rdf:datatype="http://www.w3.org/2001/XMLSchema#date">2016-06-06</dc:issued>
    <dc:modified rdf:datatype="http://www.w3.org/2001/XMLSchema#date">2016-06-06</dc:modified>
  </rdf:Property>

  <rdf:Property rdf:about="http://w3id.org/art/terms/1.0/region">
    <rdfs:label xml:lang="en">region</rdfs:label>
    <rdfs:comment xml:lang="en">Specifies the shape and location of something in Euclidean space.</rdfs:comment>
    <rdfs:isDefinedBy rdf:resource="http://w3id.org/art/terms/1.0/"/>
    <rdfs:range rdf:resource="http://www.opengis.net/ont/geosparql#Geometry"/>
    <dc:issued rdf:datatype="http://www.w3.org/2001/XMLSchema#date">2016-06-06</dc:issued>
    <dc:modified rdf:datatype="http://www.w3.org/2001/XMLSchema#date">2016-06-06</dc:modified>
  </rdf:Property>

  <rdf:Property rdf:about="http://w3id.org/art/terms/1.0/renderedAs">
    <rdfs:label xml:lang="en">renderedAs</rdfs:label>
    <rdfs:comment xml:lang="en">A rasterized portion of an image that provides bitmap data for an entity influence.</rdfs:comment>
    <rdfs:isDefinedBy rdf:resource="http://w3id.org/art/terms/1.0/"/>
    <rdfs:range rdf:resource="http://www.opengis.net/ont/geosparql#Geometry"/>
    <skos:note xml:lang="en">Artivity may record bitmap data for every influence to a document. The bitmaps are stored in PNG files and may either contain a rendering of the whole image (art:RenderingDataObject) or only of the parts (art:PartialRenderingDataObject) that have been changed. For the latter it may be required to define along a position and the extents of the parts that have changed.</skos:note>
    <dc:issued rdf:datatype="http://www.w3.org/2001/XMLSchema#date">2016-06-06</dc:issued>
    <dc:modified rdf:datatype="http://www.w3.org/2001/XMLSchema#date">2016-06-06</dc:modified>
  </rdf:Property>

  <rdf:Property rdf:about="http://w3id.org/art/terms/1.0/reverted">
    <rdfs:label xml:lang="en">reverted</rdfs:label>
    <rdfs:comment xml:lang="en">Indicates that a entity influence invalidated another.</rdfs:comment>
    <rdfs:isDefinedBy rdf:resource="http://w3id.org/art/terms/1.0/"/>
    <rdfs:range rdf:resource="http://www.w3.org/ns/prov#EntityInfluence"/>
    <rdfs:domain rdf:resource="http://www.w3.org/ns/prov#EntityInfluence"/>
    <dc:issued rdf:datatype="http://www.w3.org/2001/XMLSchema#date">2016-06-06</dc:issued>
    <dc:modified rdf:datatype="http://www.w3.org/2001/XMLSchema#date">2016-06-06</dc:modified>
  </rdf:Property>

  <rdf:Property rdf:about="http://w3id.org/art/terms/1.0/restored">
    <rdfs:label xml:lang="en">restored</rdfs:label>
    <rdfs:comment xml:lang="en">Indicates that a entity influence re-generated another.</rdfs:comment>
    <rdfs:isDefinedBy rdf:resource="http://w3id.org/art/terms/1.0/"/>
    <rdfs:range rdf:resource="http://www.w3.org/ns/prov#EntityInfluence"/>
    <rdfs:domain rdf:resource="http://www.w3.org/ns/prov#EntityInfluence"/>
    <dc:issued rdf:datatype="http://www.w3.org/2001/XMLSchema#date">2016-06-06</dc:issued>
    <dc:modified rdf:datatype="http://www.w3.org/2001/XMLSchema#date">2016-06-06</dc:modified>
  </rdf:Property>

  <rdf:Property rdf:about="http://w3id.org/art/terms/1.0/selectedGroup">
    <rdfs:label xml:lang="en">selectedGroup</rdfs:label>
    <rdfs:comment xml:lang="en">Marks a group of entities as selected within a given context.</rdfs:comment>
    <rdfs:isDefinedBy rdf:resource="http://w3id.org/art/terms/1.0/"/>
    <rdfs:domain rdf:resource="http://www.w3.org/ns/prov#EntityInfluence"/>
    <rdfs:range rdf:resource="http://w3id.org/art/terms/1.0/EntityGroup"/>
    <dc:issued rdf:datatype="http://www.w3.org/2001/XMLSchema#date">2016-06-06</dc:issued>
    <dc:modified rdf:datatype="http://www.w3.org/2001/XMLSchema#date">2016-06-06</dc:modified>
  </rdf:Property>

  <rdf:Property rdf:about="http://w3id.org/art/terms/1.0/selectedLayer">
    <rdfs:label xml:lang="en">selectedLayer</rdfs:label>
    <rdfs:comment xml:lang="en">Marks a layer as selected within a given context.</rdfs:comment>
    <rdfs:isDefinedBy rdf:resource="http://w3id.org/art/terms/1.0/"/>
    <rdfs:domain rdf:resource="http://www.w3.org/ns/prov#EntityInfluence"/>
    <rdfs:range rdf:resource="http://w3id.org/art/terms/1.0/Layer"/>
    <dc:issued rdf:datatype="http://www.w3.org/2001/XMLSchema#date">2016-06-06</dc:issued>
    <dc:modified rdf:datatype="http://www.w3.org/2001/XMLSchema#date">2016-06-06</dc:modified>
  </rdf:Property>

  <rdf:Property rdf:about="http://w3id.org/art/terms/1.0/transformationMatrix">
    <rdfs:label xml:lang="en">transformationMatrix</rdfs:label>
    <rdfs:comment xml:lang="en">Defines the basis of a vector space or a linear transformation in form of a set of vectors which are represented by a matrix.</rdfs:comment>
    <rdfs:isDefinedBy rdf:resource="http://w3id.org/art/terms/1.0/"/>
    <rdfs:seeAlso rdf:resource="https://en.wikipedia.org/wiki/Change_of_basis#Matrix_of_a_set_of_vectors"/>
    <rdfs:seeAlso rdf:resource="https://en.wikipedia.org/wiki/Transformation_matrix"/>
    <rdfs:domain rdf:resource="http://www.opengis.net/ont/geosparql#Geometry"/>
    <rdfs:domain rdf:resource="http://w3id.org/art/terms/1.0/CoordinateSystem"/>
    <rdfs:range rdf:resource="http://www.w3.org/2001/XMLSchema#string"/>
    <dc:issued rdf:datatype="http://www.w3.org/2001/XMLSchema#date">2016-06-06</dc:issued>
    <dc:modified rdf:datatype="http://www.w3.org/2001/XMLSchema#date">2016-06-06</dc:modified>
  </rdf:Property>

  <rdf:Property rdf:about="http://w3id.org/art/terms/1.0/viewport">
    <rdfs:label xml:lang="en">viewport</rdfs:label>
    <rdfs:comment xml:lang="en">References a rectangle that represents the visible area of a document.</rdfs:comment>
    <rdfs:isDefinedBy rdf:resource="http://w3id.org/art/terms/1.0/"/>
    <rdfs:domain rdf:resource="http://www.w3.org/ns/prov#EntityInfluence"/>
    <rdfs:range rdf:resource="http://w3id.org/art/terms/1.0/Viewport"/>
    <dc:issued rdf:datatype="http://www.w3.org/2001/XMLSchema#date">2016-06-06</dc:issued>
    <dc:modified rdf:datatype="http://www.w3.org/2001/XMLSchema#date">2016-06-06</dc:modified>
  </rdf:Property>

  <rdf:Property rdf:about="http://w3id.org/art/terms/1.0/width">
    <rdfs:label xml:lang="en">width</rdfs:label>
    <rdfs:comment xml:lang="en">The extents of a geometry along the x-axis of a Cartesian coordinate system.</rdfs:comment>
    <rdfs:isDefinedBy rdf:resource="http://w3id.org/art/terms/1.0/"/>
    <rdfs:domain rdf:resource="http://www.opengis.net/ont/geosparql#Geometry"/>
    <rdfs:range rdf:resource="http://www.w3.org/2001/XMLSchema#double"/>
    <dc:issued rdf:datatype="http://www.w3.org/2001/XMLSchema#date">2016-06-06</dc:issued>
    <dc:modified rdf:datatype="http://www.w3.org/2001/XMLSchema#date">2016-06-06</dc:modified>
  </rdf:Property>

  <rdf:Property rdf:about="http://w3id.org/art/terms/1.0/x">
    <rdfs:label xml:lang="en">x</rdfs:label>
    <rdfs:comment xml:lang="en">The x-coordinate value describing the position of a point in a Cartesian coordinate system.</rdfs:comment>
    <rdfs:isDefinedBy rdf:resource="http://w3id.org/art/terms/1.0/"/>
    <rdfs:domain rdf:resource="http://w3id.org/art/terms/1.0/Point"/>
    <rdfs:range rdf:resource="http://www.w3.org/2001/XMLSchema#double"/>
    <dc:issued rdf:datatype="http://www.w3.org/2001/XMLSchema#date">2016-06-06</dc:issued>
    <dc:modified rdf:datatype="http://www.w3.org/2001/XMLSchema#date">2016-06-06</dc:modified>
  </rdf:Property>

  <rdf:Property rdf:about="http://w3id.org/art/terms/1.0/y">
    <rdfs:label xml:lang="en">y</rdfs:label>
    <rdfs:comment xml:lang="en">The y-coordinate value describing the position of a point in a Cartesian coordinate system.</rdfs:comment>
    <rdfs:isDefinedBy rdf:resource="http://w3id.org/art/terms/1.0/"/>
    <rdfs:domain rdf:resource="http://w3id.org/art/terms/1.0/Point"/>
    <rdfs:range rdf:resource="http://www.w3.org/2001/XMLSchema#double"/>
    <dc:issued rdf:datatype="http://www.w3.org/2001/XMLSchema#date">2016-06-06</dc:issued>
    <dc:modified rdf:datatype="http://www.w3.org/2001/XMLSchema#date">2016-06-06</dc:modified>
  </rdf:Property>

  <rdf:Property rdf:about="http://w3id.org/art/terms/1.0/z">
    <rdfs:label xml:lang="en">z</rdfs:label>
    <rdfs:comment xml:lang="en">The z-coordinate value describing the position of a point in a Cartesian coordinate system.</rdfs:comment>
    <rdfs:isDefinedBy rdf:resource="http://w3id.org/art/terms/1.0/"/>
    <rdfs:domain rdf:resource="http://w3id.org/art/terms/1.0/Point"/>
    <rdfs:range rdf:resource="http://www.w3.org/2001/XMLSchema#double"/>
    <dc:issued rdf:datatype="http://www.w3.org/2001/XMLSchema#date">2016-06-06</dc:issued>
    <dc:modified rdf:datatype="http://www.w3.org/2001/XMLSchema#date">2016-06-06</dc:modified>
  </rdf:Property>

  <rdf:Property rdf:about="http://w3id.org/art/terms/1.0/zoomFactor">
    <rdfs:label xml:lang="en">zoomFactor</rdfs:label>
    <rdfs:comment xml:lang="en">An application specific value describing the magnification of the currently viewed geometries.</rdfs:comment>
    <rdfs:isDefinedBy rdf:resource="http://w3id.org/art/terms/1.0/"/>
    <rdfs:domain rdf:resource="http://w3id.org/art/terms/1.0/Viewport"/>
    <rdfs:range rdf:resource="http://www.w3.org/2001/XMLSchema#double"/>
    <dc:issued rdf:datatype="http://www.w3.org/2001/XMLSchema#date">2016-06-06</dc:issued>
    <dc:modified rdf:datatype="http://www.w3.org/2001/XMLSchema#date">2016-06-06</dc:modified>
  </rdf:Property>

  <rdf:Description rdf:about="http://w3id.org/art/terms/1.0/cm">
    <rdf:type rdf:resource="http://w3id.org/art/terms/1.0/LengthUnit"/>
    <rdfs:label xml:lang="en">cm</rdfs:label>
    <rdfs:comment xml:lang="en">A unit of length in the metric system, equal to one hundredth of a metre.</rdfs:comment>
    <rdfs:isDefinedBy rdf:resource="http://w3id.org/art/terms/1.0/"/>
    <rdfs:seeAlso rdf:resource="https://en.wikipedia.org/wiki/Centimetre"/>
    <dc:issued rdf:datatype="http://www.w3.org/2001/XMLSchema#date">2016-06-06</dc:issued>
    <dc:modified rdf:datatype="http://www.w3.org/2001/XMLSchema#date">2016-06-06</dc:modified>
  </rdf:Description>

  <rdf:Description rdf:about="http://w3id.org/art/terms/1.0/ft">
    <rdf:type rdf:resource="http://w3id.org/art/terms/1.0/LengthUnit"/>
    <rdfs:label xml:lang="en">ft</rdfs:label>
    <rdfs:comment xml:lang="en">A unit of length in the imperial and US customary systems of measurement. Since 1959, the international foot was defined as 0.3048 Wikipedia: meters exactly.</rdfs:comment>
    <rdfs:isDefinedBy rdf:resource="http://w3id.org/art/terms/1.0/"/>
    <rdfs:seeAlso rdf:resource="https://en.wikipedia.org/wiki/Foot_(unit)"/>
    <dc:issued rdf:datatype="http://www.w3.org/2001/XMLSchema#date">2016-06-06</dc:issued>
    <dc:modified rdf:datatype="http://www.w3.org/2001/XMLSchema#date">2016-06-06</dc:modified>
  </rdf:Description>

  <rdf:Description rdf:about="http://w3id.org/art/terms/1.0/in">
    <rdf:type rdf:resource="http://w3id.org/art/terms/1.0/LengthUnit"/>
    <rdfs:label xml:lang="en">in</rdfs:label>
    <rdfs:comment xml:lang="en">A unit of length in the imperial and US customary systems of measurement. Since 1959, the international yard was defined as 0.9144 metres exactly.</rdfs:comment>
    <rdfs:isDefinedBy rdf:resource="http://w3id.org/art/terms/1.0/"/>
    <rdfs:seeAlso rdf:resource="https://en.wikipedia.org/wiki/Inch"/>
    <dc:issued rdf:datatype="http://www.w3.org/2001/XMLSchema#date">2016-06-06</dc:issued>
    <dc:modified rdf:datatype="http://www.w3.org/2001/XMLSchema#date">2016-06-06</dc:modified>
  </rdf:Description>

  <rdf:Description rdf:about="http://w3id.org/art/terms/1.0/m">
    <rdf:type rdf:resource="http://w3id.org/art/terms/1.0/LengthUnit"/>
    <rdfs:label xml:lang="en">m</rdfs:label>
    <rdfs:comment xml:lang="en">The base unit of length in the International System of Units (SI), the modern form of the metric system.</rdfs:comment>
    <rdfs:isDefinedBy rdf:resource="http://w3id.org/art/terms/1.0/"/>
    <rdfs:seeAlso rdf:resource="https://en.wikipedia.org/wiki/Metre"/>
    <dc:issued rdf:datatype="http://www.w3.org/2001/XMLSchema#date">2016-06-06</dc:issued>
    <dc:modified rdf:datatype="http://www.w3.org/2001/XMLSchema#date">2016-06-06</dc:modified>
  </rdf:Description>

  <rdf:Description rdf:about="http://w3id.org/art/terms/1.0/mm">
    <rdf:type rdf:resource="http://w3id.org/art/terms/1.0/LengthUnit"/>
    <rdfs:label xml:lang="en">mm</rdfs:label>
    <rdfs:comment xml:lang="en">A unit of length in the metric system, equal to one thousandth of a metre.</rdfs:comment>
    <rdfs:isDefinedBy rdf:resource="http://w3id.org/art/terms/1.0/"/>
    <rdfs:seeAlso rdf:resource="https://en.wikipedia.org/wiki/Millimetre"/>
    <dc:issued rdf:datatype="http://www.w3.org/2001/XMLSchema#date">2016-06-06</dc:issued>
    <dc:modified rdf:datatype="http://www.w3.org/2001/XMLSchema#date">2016-06-06</dc:modified>
  </rdf:Description>

  <rdf:Description rdf:about="http://w3id.org/art/terms/1.0/pt">
    <rdf:type rdf:resource="http://w3id.org/art/terms/1.0/LengthUnit"/>
    <rdfs:label xml:lang="en">pt</rdfs:label>
    <rdfs:comment xml:lang="en">The smallest unit of measure in typography. The desktop publishing point is defined as 1⁄72 of an international inch (about 0.353 mm).</rdfs:comment>
    <rdfs:isDefinedBy rdf:resource="http://w3id.org/art/terms/1.0/"/>
    <rdfs:seeAlso rdf:resource="https://en.wikipedia.org/wiki/Point_(typography)"/>
    <dc:issued rdf:datatype="http://www.w3.org/2001/XMLSchema#date">2016-06-06</dc:issued>
    <dc:modified rdf:datatype="http://www.w3.org/2001/XMLSchema#date">2016-06-06</dc:modified>
  </rdf:Description>

  <rdf:Description rdf:about="http://w3id.org/art/terms/1.0/px">
    <rdf:type rdf:resource="http://w3id.org/art/terms/1.0/LengthUnit"/>
    <rdfs:label xml:lang="en">px</rdfs:label>
    <rdfs:comment xml:lang="en">A physical point in a raster image, or the smallest addressable element in an all points addressable display device.</rdfs:comment>
    <rdfs:isDefinedBy rdf:resource="http://w3id.org/art/terms/1.0/"/>
    <rdfs:seeAlso rdf:resource="https://en.wikipedia.org/wiki/Pixel"/>
    <dc:issued rdf:datatype="http://www.w3.org/2001/XMLSchema#date">2016-06-06</dc:issued>
    <dc:modified rdf:datatype="http://www.w3.org/2001/XMLSchema#date">2016-06-06</dc:modified>
  </rdf:Description>

</rdf:RDF>